feat: Add AWS KMS Hierarchical Keyring  (#109)

AwsCryptographicMaterialProviders/runtimes/java/src/main/smithy-generated/software/amazon/cryptography/materialProviders/ToDafny.java
@@ -3,16 +3,79 @@
 // Do not modify this file. This file is machine generated, and any changes to it will be overwritten.
 package software.amazon.cryptography.materialProviders;
 
-import Dafny.Aws.Cryptography.MaterialProviders.Types.*;
+import Dafny.Aws.Cryptography.MaterialProviders.Types.AesWrappingAlg;
+import Dafny.Aws.Cryptography.MaterialProviders.Types.AlgorithmSuiteId;
+import Dafny.Aws.Cryptography.MaterialProviders.Types.AlgorithmSuiteInfo;
+import Dafny.Aws.Cryptography.MaterialProviders.Types.CommitmentPolicy;
+import Dafny.Aws.Cryptography.MaterialProviders.Types.CreateAwsKmsDiscoveryKeyringInput;
+import Dafny.Aws.Cryptography.MaterialProviders.Types.CreateAwsKmsDiscoveryMultiKeyringInput;
+import Dafny.Aws.Cryptography.MaterialProviders.Types.CreateAwsKmsHierarchicalKeyringInput;
+import Dafny.Aws.Cryptography.MaterialProviders.Types.CreateAwsKmsKeyringInput;
+import Dafny.Aws.Cryptography.MaterialProviders.Types.CreateAwsKmsMrkDiscoveryKeyringInput;
+import Dafny.Aws.Cryptography.MaterialProviders.Types.CreateAwsKmsMrkDiscoveryMultiKeyringInput;
+import Dafny.Aws.Cryptography.MaterialProviders.Types.CreateAwsKmsMrkKeyringInput;
+import Dafny.Aws.Cryptography.MaterialProviders.Types.CreateAwsKmsMrkMultiKeyringInput;
+import Dafny.Aws.Cryptography.MaterialProviders.Types.CreateAwsKmsMultiKeyringInput;
+import Dafny.Aws.Cryptography.MaterialProviders.Types.CreateAwsKmsRsaKeyringInput;
+import Dafny.Aws.Cryptography.MaterialProviders.Types.CreateDefaultClientSupplierInput;
+import Dafny.Aws.Cryptography.MaterialProviders.Types.CreateDefaultCryptographicMaterialsManagerInput;
+import Dafny.Aws.Cryptography.MaterialProviders.Types.CreateMultiKeyringInput;
+import Dafny.Aws.Cryptography.MaterialProviders.Types.CreateRawAesKeyringInput;
+import Dafny.Aws.Cryptography.MaterialProviders.Types.CreateRawRsaKeyringInput;
+import Dafny.Aws.Cryptography.MaterialProviders.Types.DBEAlgorithmSuiteId;
+import Dafny.Aws.Cryptography.MaterialProviders.Types.DBECommitmentPolicy;
+import Dafny.Aws.Cryptography.MaterialProviders.Types.DIRECT__KEY__WRAPPING;
+import Dafny.Aws.Cryptography.MaterialProviders.Types.DecryptMaterialsInput;
+import Dafny.Aws.Cryptography.MaterialProviders.Types.DecryptMaterialsOutput;
+import Dafny.Aws.Cryptography.MaterialProviders.Types.DecryptionMaterials;
+import Dafny.Aws.Cryptography.MaterialProviders.Types.DerivationAlgorithm;
+import Dafny.Aws.Cryptography.MaterialProviders.Types.DiscoveryFilter;
+import Dafny.Aws.Cryptography.MaterialProviders.Types.ECDSA;
+import Dafny.Aws.Cryptography.MaterialProviders.Types.ESDKAlgorithmSuiteId;
+import Dafny.Aws.Cryptography.MaterialProviders.Types.ESDKCommitmentPolicy;
+import Dafny.Aws.Cryptography.MaterialProviders.Types.EdkWrappingAlgorithm;
+import Dafny.Aws.Cryptography.MaterialProviders.Types.Encrypt;
+import Dafny.Aws.Cryptography.MaterialProviders.Types.EncryptedDataKey;
+import Dafny.Aws.Cryptography.MaterialProviders.Types.EncryptionMaterials;
 import Dafny.Aws.Cryptography.MaterialProviders.Types.Error;
+import Dafny.Aws.Cryptography.MaterialProviders.Types.Error_AwsCryptographicMaterialProvidersException;
+import Dafny.Aws.Cryptography.MaterialProviders.Types.Error_InvalidAlgorithmSuiteInfo;
+import Dafny.Aws.Cryptography.MaterialProviders.Types.Error_InvalidAlgorithmSuiteInfoOnDecrypt;
+import Dafny.Aws.Cryptography.MaterialProviders.Types.Error_InvalidAlgorithmSuiteInfoOnEncrypt;
+import Dafny.Aws.Cryptography.MaterialProviders.Types.Error_InvalidDecryptionMaterials;
+import Dafny.Aws.Cryptography.MaterialProviders.Types.Error_InvalidDecryptionMaterialsTransition;
+import Dafny.Aws.Cryptography.MaterialProviders.Types.Error_InvalidEncryptionMaterials;
+import Dafny.Aws.Cryptography.MaterialProviders.Types.Error_InvalidEncryptionMaterialsTransition;
+import Dafny.Aws.Cryptography.MaterialProviders.Types.GetClientInput;
+import Dafny.Aws.Cryptography.MaterialProviders.Types.GetEncryptionMaterialsInput;
+import Dafny.Aws.Cryptography.MaterialProviders.Types.GetEncryptionMaterialsOutput;
+import Dafny.Aws.Cryptography.MaterialProviders.Types.HKDF;
+import Dafny.Aws.Cryptography.MaterialProviders.Types.HierarchicalMaterials;
 import Dafny.Aws.Cryptography.MaterialProviders.Types.IClientSupplier;
-import Dafny.Aws.Cryptography.MaterialProviders.Types.ICryptographicMaterialsManager;
+import Dafny.Aws.Cryptography.MaterialProviders.Types.IDENTITY;
 import Dafny.Aws.Cryptography.MaterialProviders.Types.IKeyring;
+import Dafny.Aws.Cryptography.MaterialProviders.Types.ICryptographicMaterialsManager;
+import Dafny.Aws.Cryptography.MaterialProviders.Types.InitializeDecryptionMaterialsInput;
+import Dafny.Aws.Cryptography.MaterialProviders.Types.InitializeEncryptionMaterialsInput;
+import Dafny.Aws.Cryptography.MaterialProviders.Types.IntermediateKeyWrapping;
+import Dafny.Aws.Cryptography.MaterialProviders.Types.MaterialProvidersConfig;
+import Dafny.Aws.Cryptography.MaterialProviders.Types.None;
+import Dafny.Aws.Cryptography.MaterialProviders.Types.OnDecryptInput;
+import Dafny.Aws.Cryptography.MaterialProviders.Types.OnDecryptOutput;
+import Dafny.Aws.Cryptography.MaterialProviders.Types.OnEncryptInput;
+import Dafny.Aws.Cryptography.MaterialProviders.Types.OnEncryptOutput;
+import Dafny.Aws.Cryptography.MaterialProviders.Types.PaddingScheme;
+import Dafny.Aws.Cryptography.MaterialProviders.Types.SignatureAlgorithm;
+import Dafny.Aws.Cryptography.MaterialProviders.Types.SymmetricSignatureAlgorithm;
+import Dafny.Aws.Cryptography.MaterialProviders.Types.ValidDecryptionMaterialsTransitionInput;
+import Dafny.Aws.Cryptography.MaterialProviders.Types.ValidEncryptionMaterialsTransitionInput;
+import Dafny.Aws.Cryptography.MaterialProviders.Types.ValidateCommitmentPolicyOnDecryptInput;
+import Dafny.Aws.Cryptography.MaterialProviders.Types.ValidateCommitmentPolicyOnEncryptInput;
 import Dafny.Aws.Cryptography.Primitives.Types.DigestAlgorithm;
 import Dafny.Aws.Cryptography.Primitives.Types.ECDSASignatureAlgorithm;
 import Dafny.Com.Amazonaws.Dynamodb.Types.IDynamoDB__20120810Client;
-import Dafny.Com.Amazonaws.Kms.Types.IKeyManagementServiceClient;
 import Dafny.Com.Amazonaws.Kms.Types.EncryptionAlgorithmSpec;
+import Dafny.Com.Amazonaws.Kms.Types.IKeyManagementServiceClient;
 import Wrappers_Compile.Option;
 import dafny.DafnyMap;
 import dafny.DafnySequence;
@@ -28,8 +91,10 @@ import java.nio.ByteBuffer;
 import java.util.List;
 import java.util.Map;
 import java.util.Objects;
+import java.util.function.Function;
 import software.amazon.cryptography.materialProviders.model.AwsCryptographicMaterialProvidersException;
 import software.amazon.cryptography.materialProviders.model.CollectionOfErrors;
+import software.amazon.cryptography.materialProviders.model.DIRECT_KEY_WRAPPING;
 import software.amazon.cryptography.materialProviders.model.InvalidAlgorithmSuiteInfo;
 import software.amazon.cryptography.materialProviders.model.InvalidAlgorithmSuiteInfoOnDecrypt;
 import software.amazon.cryptography.materialProviders.model.InvalidAlgorithmSuiteInfoOnEncrypt;
@@ -39,33 +104,32 @@ import software.amazon.cryptography.materialProviders.model.InvalidEncryptionMat
 import software.amazon.cryptography.materialProviders.model.InvalidEncryptionMaterialsTransition;
 import software.amazon.cryptography.materialProviders.model.NativeError;
 import software.amazon.cryptography.materialProviders.model.OpaqueError;
-import software.amazon.cryptography.materialProviders.model.DIRECT_KEY_WRAPPING;
 
 public class ToDafny {
   public static Error Error(NativeError nativeValue) {
+    if (nativeValue instanceof InvalidDecryptionMaterialsTransition) {
+      return ToDafny.Error((InvalidDecryptionMaterialsTransition) nativeValue);
+    }
+    if (nativeValue instanceof InvalidAlgorithmSuiteInfoOnDecrypt) {
+      return ToDafny.Error((InvalidAlgorithmSuiteInfoOnDecrypt) nativeValue);
+    }
     if (nativeValue instanceof InvalidDecryptionMaterials) {
       return ToDafny.Error((InvalidDecryptionMaterials) nativeValue);
     }
     if (nativeValue instanceof InvalidAlgorithmSuiteInfo) {
       return ToDafny.Error((InvalidAlgorithmSuiteInfo) nativeValue);
     }
+    if (nativeValue instanceof AwsCryptographicMaterialProvidersException) {
+      return ToDafny.Error((AwsCryptographicMaterialProvidersException) nativeValue);
+    }
+    if (nativeValue instanceof InvalidEncryptionMaterialsTransition) {
+      return ToDafny.Error((InvalidEncryptionMaterialsTransition) nativeValue);
+    }
     if (nativeValue instanceof InvalidAlgorithmSuiteInfoOnEncrypt) {
       return ToDafny.Error((InvalidAlgorithmSuiteInfoOnEncrypt) nativeValue);
     }
     if (nativeValue instanceof InvalidEncryptionMaterials) {
       return ToDafny.Error((InvalidEncryptionMaterials) nativeValue);
-    }
-    if (nativeValue instanceof InvalidDecryptionMaterialsTransition) {
-      return ToDafny.Error((InvalidDecryptionMaterialsTransition) nativeValue);
-    }
-    if (nativeValue instanceof InvalidEncryptionMaterialsTransition) {
-      return ToDafny.Error((InvalidEncryptionMaterialsTransition) nativeValue);
-    }
-    if (nativeValue instanceof InvalidAlgorithmSuiteInfoOnDecrypt) {
-      return ToDafny.Error((InvalidAlgorithmSuiteInfoOnDecrypt) nativeValue);
-    }
-    if (nativeValue instanceof AwsCryptographicMaterialProvidersException) {
-      return ToDafny.Error((AwsCryptographicMaterialProvidersException) nativeValue);
     }
     if (nativeValue instanceof OpaqueError) {
       return ToDafny.Error((OpaqueError) nativeValue);
@@ -88,11 +152,44 @@ public class ToDafny {
     return Error.create_Collection(list);
   }
 
-  public static OnEncryptInput OnEncryptInput(
-      software.amazon.cryptography.materialProviders.model.OnEncryptInput nativeValue) {
-    EncryptionMaterials materials;
-    materials = ToDafny.EncryptionMaterials(nativeValue.materials());
-    return new OnEncryptInput(materials);
+  public static CreateDefaultClientSupplierInput CreateDefaultClientSupplierInput(
+      software.amazon.cryptography.materialProviders.model.CreateDefaultClientSupplierInput nativeValue) {
+    return new CreateDefaultClientSupplierInput();
+  }
+
+  public static IDENTITY IDENTITY(
+      software.amazon.cryptography.materialProviders.model.IDENTITY nativeValue) {
+    return new IDENTITY();
+  }
+
+  public static CreateAwsKmsMrkMultiKeyringInput CreateAwsKmsMrkMultiKeyringInput(
+      software.amazon.cryptography.materialProviders.model.CreateAwsKmsMrkMultiKeyringInput nativeValue) {
+    Option<DafnySequence<? extends Character>> generator;
+    generator = Objects.nonNull(nativeValue.generator()) ?
+        Option.create_Some(software.amazon.dafny.conversion.ToDafny.Simple.CharacterSequence(nativeValue.generator()))
+        : Option.create_None();
+    Option<DafnySequence<? extends DafnySequence<? extends Character>>> kmsKeyIds;
+    kmsKeyIds = Objects.nonNull(nativeValue.kmsKeyIds()) ?
+        Option.create_Some(ToDafny.KmsKeyIdList(nativeValue.kmsKeyIds()))
+        : Option.create_None();
+    Option<IClientSupplier> clientSupplier;
+    clientSupplier = Objects.nonNull(nativeValue.clientSupplier()) ?
+            Option.create_Some(ToDafny.ClientSupplier(nativeValue.clientSupplier()))
+            : Option.create_None();
+    Option<DafnySequence<? extends DafnySequence<? extends Character>>> grantTokens;
+    grantTokens = Objects.nonNull(nativeValue.grantTokens()) ?
+        Option.create_Some(ToDafny.GrantTokenList(nativeValue.grantTokens()))
+        : Option.create_None();
+    return new CreateAwsKmsMrkMultiKeyringInput(generator, kmsKeyIds, clientSupplier, grantTokens);
+  }
+
+  public static ValidateCommitmentPolicyOnEncryptInput ValidateCommitmentPolicyOnEncryptInput(
+      software.amazon.cryptography.materialProviders.model.ValidateCommitmentPolicyOnEncryptInput nativeValue) {
+    AlgorithmSuiteId algorithm;
+    algorithm = ToDafny.AlgorithmSuiteId(nativeValue.algorithm());
+    CommitmentPolicy commitmentPolicy;
+    commitmentPolicy = ToDafny.CommitmentPolicy(nativeValue.commitmentPolicy());
+    return new ValidateCommitmentPolicyOnEncryptInput(algorithm, commitmentPolicy);
   }
 
   public static CreateAwsKmsKeyringInput CreateAwsKmsKeyringInput(
@@ -103,152 +200,102 @@ public class ToDafny {
     kmsClient = new Dafny.Com.Amazonaws.Kms.Shim(nativeValue.kmsClient(), null);
     Option<DafnySequence<? extends DafnySequence<? extends Character>>> grantTokens;
     grantTokens = Objects.nonNull(nativeValue.grantTokens()) ?
-        Option.create_Some(ToDafny.GrantTokenList(nativeValue.grantTokens()))
-        : Option.create_None();
+            Option.create_Some(ToDafny.GrantTokenList(nativeValue.grantTokens()))
+            : Option.create_None();
     return new CreateAwsKmsKeyringInput(kmsKeyId, kmsClient, grantTokens);
   }
 
-  public static GetEncryptionMaterialsOutput GetEncryptionMaterialsOutput(
-      software.amazon.cryptography.materialProviders.model.GetEncryptionMaterialsOutput nativeValue) {
-    EncryptionMaterials encryptionMaterials;
-    encryptionMaterials = ToDafny.EncryptionMaterials(nativeValue.encryptionMaterials());
-    return new GetEncryptionMaterialsOutput(encryptionMaterials);
-  }
-
-  public static CreateAwsKmsMrkDiscoveryKeyringInput CreateAwsKmsMrkDiscoveryKeyringInput(
-      software.amazon.cryptography.materialProviders.model.CreateAwsKmsMrkDiscoveryKeyringInput nativeValue) {
-    IKeyManagementServiceClient kmsClient;
-    kmsClient = new Dafny.Com.Amazonaws.Kms.Shim(nativeValue.kmsClient(), null);
-    Option<DiscoveryFilter> discoveryFilter;
-    discoveryFilter = Objects.nonNull(nativeValue.discoveryFilter()) ?
-        Option.create_Some(ToDafny.DiscoveryFilter(nativeValue.discoveryFilter()))
-        : Option.create_None();
-    Option<DafnySequence<? extends DafnySequence<? extends Character>>> grantTokens;
-    grantTokens = Objects.nonNull(nativeValue.grantTokens()) ?
-        Option.create_Some(ToDafny.GrantTokenList(nativeValue.grantTokens()))
-        : Option.create_None();
+  public static GetClientInput GetClientInput(
+      software.amazon.cryptography.materialProviders.model.GetClientInput nativeValue) {
     DafnySequence<? extends Character> region;
     region = software.amazon.dafny.conversion.ToDafny.Simple.CharacterSequence(nativeValue.region());
-    return new CreateAwsKmsMrkDiscoveryKeyringInput(kmsClient, discoveryFilter, grantTokens, region);
+    return new GetClientInput(region);
   }
 
-
-  public static CreateAwsKmsHierarchicalKeyringInput CreateAwsKmsHierarchyKeyringInput(
-          software.amazon.cryptography.materialProviders.model.CreateAwsKmsHierarchicalKeyringInput nativeValue) {
-    DafnySequence<? extends Character> branchKeyId;
-    branchKeyId = software.amazon.dafny.conversion.ToDafny.Simple.CharacterSequence(nativeValue.branchKeyId());
-    DafnySequence<? extends Character> kmsKeyId;
-    kmsKeyId = software.amazon.dafny.conversion.ToDafny.Simple.CharacterSequence(nativeValue.kmsKeyId());
-    IKeyManagementServiceClient kmsClient;
-    kmsClient = new Dafny.Com.Amazonaws.Kms.Shim(nativeValue.kmsClient(), null);
-    IDynamoDB__20120810Client ddbClient;
-    ddbClient = new Dafny.Com.Amazonaws.Dynamodb.Shim(nativeValue.ddbClient(), null);
-    DafnySequence<? extends Character> branchKeysTableName;
-    branchKeysTableName = software.amazon.dafny.conversion.ToDafny.Simple.CharacterSequence(nativeValue.branchKeysTableName());
-    Long ttlMilliseconds;
-    ttlMilliseconds = (nativeValue.ttlMilliseconds());
-    Option<Integer> maxCacheSize;
-    maxCacheSize = Objects.nonNull(nativeValue.maxCacheSize()) ?
-            Option.create_Some((nativeValue.maxCacheSize()))
-            : Option.create_None();
-    Option<DafnySequence<? extends DafnySequence<? extends Character>>> grantTokens;
-    grantTokens = Objects.nonNull(nativeValue.grantTokens()) ?
-            Option.create_Some(ToDafny.GrantTokenList(nativeValue.grantTokens()))
-            : Option.create_None();
-    return new CreateAwsKmsHierarchicalKeyringInput(branchKeyId, kmsKeyId, kmsClient, ddbClient, branchKeysTableName, ttlMilliseconds, maxCacheSize, grantTokens);
+  public static HierarchicalMaterials HierarchicalMaterials(
+      software.amazon.cryptography.materialProviders.model.HierarchicalMaterials nativeValue) {
+    DafnySequence<? extends Byte> branchKeyVersion;
+    branchKeyVersion = software.amazon.dafny.conversion.ToDafny.Simple.DafnyUtf8Bytes(nativeValue.branchKeyVersion());
+    DafnySequence<? extends Byte> branchKey;
+    branchKey = software.amazon.dafny.conversion.ToDafny.Simple.ByteSequence(nativeValue.branchKey());
+    return new HierarchicalMaterials(branchKeyVersion, branchKey);
   }
 
-  public static IDENTITY IDENTITY(
-      software.amazon.cryptography.materialProviders.model.IDENTITY nativeValue) {
-    return new IDENTITY();
+  public static DiscoveryFilter DiscoveryFilter(
+      software.amazon.cryptography.materialProviders.model.DiscoveryFilter nativeValue) {
+    DafnySequence<? extends DafnySequence<? extends Character>> accountIds;
+    accountIds = ToDafny.AccountIdList(nativeValue.accountIds());
+    DafnySequence<? extends Character> partition;
+    partition = software.amazon.dafny.conversion.ToDafny.Simple.CharacterSequence(nativeValue.partition());
+    return new DiscoveryFilter(accountIds, partition);
   }
 
-  public static CreateAwsKmsMrkKeyringInput CreateAwsKmsMrkKeyringInput(
-      software.amazon.cryptography.materialProviders.model.CreateAwsKmsMrkKeyringInput nativeValue) {
-    DafnySequence<? extends Character> kmsKeyId;
-    kmsKeyId = software.amazon.dafny.conversion.ToDafny.Simple.CharacterSequence(nativeValue.kmsKeyId());
-    IKeyManagementServiceClient kmsClient;
-    kmsClient = new Dafny.Com.Amazonaws.Kms.Shim(nativeValue.kmsClient(), null);
-    Option<DafnySequence<? extends DafnySequence<? extends Character>>> grantTokens;
-    grantTokens = Objects.nonNull(nativeValue.grantTokens()) ?
-        Option.create_Some(ToDafny.GrantTokenList(nativeValue.grantTokens()))
-        : Option.create_None();
-    return new CreateAwsKmsMrkKeyringInput(kmsKeyId, kmsClient, grantTokens);
+  public static DecryptMaterialsOutput DecryptMaterialsOutput(
+      software.amazon.cryptography.materialProviders.model.DecryptMaterialsOutput nativeValue) {
+    DecryptionMaterials decryptionMaterials;
+    decryptionMaterials = ToDafny.DecryptionMaterials(nativeValue.decryptionMaterials());
+    return new DecryptMaterialsOutput(decryptionMaterials);
   }
 
-  public static CreateAwsKmsDiscoveryKeyringInput CreateAwsKmsDiscoveryKeyringInput(
-      software.amazon.cryptography.materialProviders.model.CreateAwsKmsDiscoveryKeyringInput nativeValue) {
-    IKeyManagementServiceClient kmsClient;
-    kmsClient = new Dafny.Com.Amazonaws.Kms.Shim(nativeValue.kmsClient(), null);
-    Option<DiscoveryFilter> discoveryFilter;
-    discoveryFilter = Objects.nonNull(nativeValue.discoveryFilter()) ?
-        Option.create_Some(ToDafny.DiscoveryFilter(nativeValue.discoveryFilter()))
-        : Option.create_None();
-    Option<DafnySequence<? extends DafnySequence<? extends Character>>> grantTokens;
-    grantTokens = Objects.nonNull(nativeValue.grantTokens()) ?
-        Option.create_Some(ToDafny.GrantTokenList(nativeValue.grantTokens()))
-        : Option.create_None();
-    return new CreateAwsKmsDiscoveryKeyringInput(kmsClient, discoveryFilter, grantTokens);
+  public static CreateDefaultCryptographicMaterialsManagerInput CreateDefaultCryptographicMaterialsManagerInput(
+      software.amazon.cryptography.materialProviders.model.CreateDefaultCryptographicMaterialsManagerInput nativeValue) {
+    IKeyring keyring;
+    keyring = ToDafny.Keyring(nativeValue.keyring());
+    return new CreateDefaultCryptographicMaterialsManagerInput(keyring);
   }
 
-  public static CreateAwsKmsRsaKeyringInput CreateAwsKmsRsaKeyringInput(
-      software.amazon.cryptography.materialProviders.model.CreateAwsKmsRsaKeyringInput nativeValue) {
+  public static CreateRawRsaKeyringInput CreateRawRsaKeyringInput(
+      software.amazon.cryptography.materialProviders.model.CreateRawRsaKeyringInput nativeValue) {
+    DafnySequence<? extends Character> keyNamespace;
+    keyNamespace = software.amazon.dafny.conversion.ToDafny.Simple.CharacterSequence(nativeValue.keyNamespace());
+    DafnySequence<? extends Character> keyName;
+    keyName = software.amazon.dafny.conversion.ToDafny.Simple.CharacterSequence(nativeValue.keyName());
+    PaddingScheme paddingScheme;
+    paddingScheme = ToDafny.PaddingScheme(nativeValue.paddingScheme());
     Option<DafnySequence<? extends Byte>> publicKey;
     publicKey = Objects.nonNull(nativeValue.publicKey()) ?
         Option.create_Some(software.amazon.dafny.conversion.ToDafny.Simple.ByteSequence(nativeValue.publicKey()))
         : Option.create_None();
-    DafnySequence<? extends Character> kmsKeyId;
-    kmsKeyId = software.amazon.dafny.conversion.ToDafny.Simple.CharacterSequence(nativeValue.kmsKeyId());
-    EncryptionAlgorithmSpec encryptionAlgorithm;
-    encryptionAlgorithm = Dafny.Com.Amazonaws.Kms.ToDafny.EncryptionAlgorithmSpec(nativeValue.encryptionAlgorithm());
-    Option<IKeyManagementServiceClient> kmsClient;
-    kmsClient = Objects.nonNull(nativeValue.kmsClient()) ?
-        Option.create_Some((new Dafny.Com.Amazonaws.Kms.Shim(nativeValue.kmsClient(), null)))
+    Option<DafnySequence<? extends Byte>> privateKey;
+    privateKey = Objects.nonNull(nativeValue.privateKey()) ?
+        Option.create_Some(software.amazon.dafny.conversion.ToDafny.Simple.ByteSequence(nativeValue.privateKey()))
         : Option.create_None();
+    return new CreateRawRsaKeyringInput(keyNamespace, keyName, paddingScheme, publicKey, privateKey);
+  }
+
+  public static OnDecryptInput OnDecryptInput(
+      software.amazon.cryptography.materialProviders.model.OnDecryptInput nativeValue) {
+    DecryptionMaterials materials;
+    materials = ToDafny.DecryptionMaterials(nativeValue.materials());
+    DafnySequence<? extends EncryptedDataKey> encryptedDataKeys;
+    encryptedDataKeys = ToDafny.EncryptedDataKeyList(nativeValue.encryptedDataKeys());
+    return new OnDecryptInput(materials, encryptedDataKeys);
+  }
+
+  public static ECDSA ECDSA(
+      software.amazon.cryptography.materialProviders.model.ECDSA nativeValue) {
+    ECDSASignatureAlgorithm curve;
+    curve = software.amazon.cryptography.primitives.ToDafny.ECDSASignatureAlgorithm(nativeValue.curve());
+    return new ECDSA(curve);
+  }
+
+  public static CreateAwsKmsMrkDiscoveryMultiKeyringInput CreateAwsKmsMrkDiscoveryMultiKeyringInput(
+      software.amazon.cryptography.materialProviders.model.CreateAwsKmsMrkDiscoveryMultiKeyringInput nativeValue) {
+    DafnySequence<? extends DafnySequence<? extends Character>> regions;
+    regions = ToDafny.RegionList(nativeValue.regions());
+    Option<DiscoveryFilter> discoveryFilter;
+    discoveryFilter = Objects.nonNull(nativeValue.discoveryFilter()) ?
+        Option.create_Some(ToDafny.DiscoveryFilter(nativeValue.discoveryFilter()))
+        : Option.create_None();
+    Option<IClientSupplier> clientSupplier;
+    clientSupplier = Objects.nonNull(nativeValue.clientSupplier()) ?
+            Option.create_Some(ToDafny.ClientSupplier(nativeValue.clientSupplier()))
+            : Option.create_None();
     Option<DafnySequence<? extends DafnySequence<? extends Character>>> grantTokens;
     grantTokens = Objects.nonNull(nativeValue.grantTokens()) ?
         Option.create_Some(ToDafny.GrantTokenList(nativeValue.grantTokens()))
         : Option.create_None();
-    return new CreateAwsKmsRsaKeyringInput(publicKey, kmsKeyId, encryptionAlgorithm, kmsClient, grantTokens);
-  }
-
-  public static ValidateCommitmentPolicyOnDecryptInput ValidateCommitmentPolicyOnDecryptInput(
-      software.amazon.cryptography.materialProviders.model.ValidateCommitmentPolicyOnDecryptInput nativeValue) {
-    AlgorithmSuiteId algorithm;
-    algorithm = ToDafny.AlgorithmSuiteId(nativeValue.algorithm());
-    CommitmentPolicy commitmentPolicy;
-    commitmentPolicy = ToDafny.CommitmentPolicy(nativeValue.commitmentPolicy());
-    return new ValidateCommitmentPolicyOnDecryptInput(algorithm, commitmentPolicy);
-  }
-
-  public static DecryptionMaterials DecryptionMaterials(
-      software.amazon.cryptography.materialProviders.model.DecryptionMaterials nativeValue) {
-    AlgorithmSuiteInfo algorithmSuite;
-    algorithmSuite = ToDafny.AlgorithmSuiteInfo(nativeValue.algorithmSuite());
-    DafnyMap<? extends DafnySequence<? extends Byte>, ? extends DafnySequence<? extends Byte>> encryptionContext;
-    encryptionContext = ToDafny.EncryptionContext(nativeValue.encryptionContext());
-    Option<DafnySequence<? extends Byte>> plaintextDataKey;
-    plaintextDataKey = Objects.nonNull(nativeValue.plaintextDataKey()) ?
-        Option.create_Some(software.amazon.dafny.conversion.ToDafny.Simple.ByteSequence(nativeValue.plaintextDataKey()))
-        : Option.create_None();
-    Option<DafnySequence<? extends Byte>> verificationKey;
-    verificationKey = Objects.nonNull(nativeValue.verificationKey()) ?
-        Option.create_Some(software.amazon.dafny.conversion.ToDafny.Simple.ByteSequence(nativeValue.verificationKey()))
-        : Option.create_None();
-    Option<DafnySequence<? extends Byte>> symmetricSigningKey;
-    symmetricSigningKey = Objects.nonNull(nativeValue.symmetricSigningKey()) ?
-        Option.create_Some(software.amazon.dafny.conversion.ToDafny.Simple.ByteSequence(nativeValue.symmetricSigningKey()))
-        : Option.create_None();
-    return new DecryptionMaterials(algorithmSuite, encryptionContext, plaintextDataKey, verificationKey, symmetricSigningKey);
-  }
-
-  public static InitializeDecryptionMaterialsInput InitializeDecryptionMaterialsInput(
-      software.amazon.cryptography.materialProviders.model.InitializeDecryptionMaterialsInput nativeValue) {
-    AlgorithmSuiteId algorithmSuiteId;
-    algorithmSuiteId = ToDafny.AlgorithmSuiteId(nativeValue.algorithmSuiteId());
-    DafnyMap<? extends DafnySequence<? extends Byte>, ? extends DafnySequence<? extends Byte>> encryptionContext;
-    encryptionContext = ToDafny.EncryptionContext(nativeValue.encryptionContext());
-    return new InitializeDecryptionMaterialsInput(algorithmSuiteId, encryptionContext);
+    return new CreateAwsKmsMrkDiscoveryMultiKeyringInput(regions, discoveryFilter, clientSupplier, grantTokens);
   }
 
   public static AlgorithmSuiteInfo AlgorithmSuiteInfo(
@@ -274,161 +321,15 @@ public class ToDafny {
     return new AlgorithmSuiteInfo(id, binaryId, messageVersion, encrypt, kdf, commitment, signature, symmetricSignature, edkWrapping);
   }
 
-  public static OnDecryptInput OnDecryptInput(
-      software.amazon.cryptography.materialProviders.model.OnDecryptInput nativeValue) {
-    DecryptionMaterials materials;
-    materials = ToDafny.DecryptionMaterials(nativeValue.materials());
-    DafnySequence<? extends EncryptedDataKey> encryptedDataKeys;
-    encryptedDataKeys = ToDafny.EncryptedDataKeyList(nativeValue.encryptedDataKeys());
-    return new OnDecryptInput(materials, encryptedDataKeys);
-  }
-
-  public static EncryptedDataKey EncryptedDataKey(
-      software.amazon.cryptography.materialProviders.model.EncryptedDataKey nativeValue) {
-    DafnySequence<? extends Byte> keyProviderId;
-    keyProviderId = software.amazon.dafny.conversion.ToDafny.Simple.DafnyUtf8Bytes(nativeValue.keyProviderId());
-    DafnySequence<? extends Byte> keyProviderInfo;
-    keyProviderInfo = software.amazon.dafny.conversion.ToDafny.Simple.ByteSequence(nativeValue.keyProviderInfo());
-    DafnySequence<? extends Byte> ciphertext;
-    ciphertext = software.amazon.dafny.conversion.ToDafny.Simple.ByteSequence(nativeValue.ciphertext());
-    return new EncryptedDataKey(keyProviderId, keyProviderInfo, ciphertext);
-  }
-
-  public static MaterialProvidersConfig MaterialProvidersConfig(
-      software.amazon.cryptography.materialProviders.model.MaterialProvidersConfig nativeValue) {
-    return new MaterialProvidersConfig();
-  }
-
-  public static ValidEncryptionMaterialsTransitionInput ValidEncryptionMaterialsTransitionInput(
-      software.amazon.cryptography.materialProviders.model.ValidEncryptionMaterialsTransitionInput nativeValue) {
-    EncryptionMaterials start;
-    start = ToDafny.EncryptionMaterials(nativeValue.start());
-    EncryptionMaterials stop;
-    stop = ToDafny.EncryptionMaterials(nativeValue.stop());
-    return new ValidEncryptionMaterialsTransitionInput(start, stop);
-  }
-
-  public static GetClientInput GetClientInput(
-      software.amazon.cryptography.materialProviders.model.GetClientInput nativeValue) {
-    DafnySequence<? extends Character> region;
-    region = software.amazon.dafny.conversion.ToDafny.Simple.CharacterSequence(nativeValue.region());
-    return new GetClientInput(region);
-  }
-
-  public static CreateRawRsaKeyringInput CreateRawRsaKeyringInput(
-      software.amazon.cryptography.materialProviders.model.CreateRawRsaKeyringInput nativeValue) {
-    DafnySequence<? extends Character> keyNamespace;
-    keyNamespace = software.amazon.dafny.conversion.ToDafny.Simple.CharacterSequence(nativeValue.keyNamespace());
-    DafnySequence<? extends Character> keyName;
-    keyName = software.amazon.dafny.conversion.ToDafny.Simple.CharacterSequence(nativeValue.keyName());
-    PaddingScheme paddingScheme;
-    paddingScheme = ToDafny.PaddingScheme(nativeValue.paddingScheme());
-    Option<DafnySequence<? extends Byte>> publicKey;
-    publicKey = Objects.nonNull(nativeValue.publicKey()) ?
-        Option.create_Some(software.amazon.dafny.conversion.ToDafny.Simple.ByteSequence(nativeValue.publicKey()))
-        : Option.create_None();
-    Option<DafnySequence<? extends Byte>> privateKey;
-    privateKey = Objects.nonNull(nativeValue.privateKey()) ?
-        Option.create_Some(software.amazon.dafny.conversion.ToDafny.Simple.ByteSequence(nativeValue.privateKey()))
-        : Option.create_None();
-    return new CreateRawRsaKeyringInput(keyNamespace, keyName, paddingScheme, publicKey, privateKey);
-  }
-
-  public static CreateDefaultCryptographicMaterialsManagerInput CreateDefaultCryptographicMaterialsManagerInput(
-      software.amazon.cryptography.materialProviders.model.CreateDefaultCryptographicMaterialsManagerInput nativeValue) {
-    IKeyring keyring;
-    keyring = ToDafny.Keyring(nativeValue.keyring());
-    return new CreateDefaultCryptographicMaterialsManagerInput(keyring);
-  }
-
-  public static GetEncryptionMaterialsInput GetEncryptionMaterialsInput(
-      software.amazon.cryptography.materialProviders.model.GetEncryptionMaterialsInput nativeValue) {
-    DafnyMap<? extends DafnySequence<? extends Byte>, ? extends DafnySequence<? extends Byte>> encryptionContext;
-    encryptionContext = ToDafny.EncryptionContext(nativeValue.encryptionContext());
-    CommitmentPolicy commitmentPolicy;
-    commitmentPolicy = ToDafny.CommitmentPolicy(nativeValue.commitmentPolicy());
-    Option<AlgorithmSuiteId> algorithmSuiteId;
-    algorithmSuiteId = Objects.nonNull(nativeValue.algorithmSuiteId()) ?
-        Option.create_Some(ToDafny.AlgorithmSuiteId(nativeValue.algorithmSuiteId()))
-        : Option.create_None();
-    Option<Long> maxPlaintextLength;
-    maxPlaintextLength = Objects.nonNull(nativeValue.maxPlaintextLength()) ?
-        Option.create_Some((nativeValue.maxPlaintextLength()))
-        : Option.create_None();
-    return new GetEncryptionMaterialsInput(encryptionContext, commitmentPolicy, algorithmSuiteId, maxPlaintextLength);
-  }
-
-  public static OnDecryptOutput OnDecryptOutput(
-      software.amazon.cryptography.materialProviders.model.OnDecryptOutput nativeValue) {
-    DecryptionMaterials materials;
-    materials = ToDafny.DecryptionMaterials(nativeValue.materials());
-    return new OnDecryptOutput(materials);
-  }
-
-  public static OnEncryptOutput OnEncryptOutput(
-      software.amazon.cryptography.materialProviders.model.OnEncryptOutput nativeValue) {
-    EncryptionMaterials materials;
-    materials = ToDafny.EncryptionMaterials(nativeValue.materials());
-    return new OnEncryptOutput(materials);
-  }
-
-  public static CreateAwsKmsMultiKeyringInput CreateAwsKmsMultiKeyringInput(
-      software.amazon.cryptography.materialProviders.model.CreateAwsKmsMultiKeyringInput nativeValue) {
-    Option<DafnySequence<? extends Character>> generator;
-    generator = Objects.nonNull(nativeValue.generator()) ?
-        Option.create_Some(software.amazon.dafny.conversion.ToDafny.Simple.CharacterSequence(nativeValue.generator()))
-        : Option.create_None();
-    Option<DafnySequence<? extends DafnySequence<? extends Character>>> kmsKeyIds;
-    kmsKeyIds = Objects.nonNull(nativeValue.kmsKeyIds()) ?
-        Option.create_Some(ToDafny.KmsKeyIdList(nativeValue.kmsKeyIds()))
-        : Option.create_None();
-    Option<IClientSupplier> clientSupplier;
-    clientSupplier = Objects.nonNull(nativeValue.clientSupplier()) ?
-        Option.create_Some(ToDafny.ClientSupplier(nativeValue.clientSupplier()))
-        : Option.create_None();
-    Option<DafnySequence<? extends DafnySequence<? extends Character>>> grantTokens;
-    grantTokens = Objects.nonNull(nativeValue.grantTokens()) ?
-        Option.create_Some(ToDafny.GrantTokenList(nativeValue.grantTokens()))
-        : Option.create_None();
-    return new CreateAwsKmsMultiKeyringInput(generator, kmsKeyIds, clientSupplier, grantTokens);
-  }
-
-  public static CreateAwsKmsDiscoveryMultiKeyringInput CreateAwsKmsDiscoveryMultiKeyringInput(
-      software.amazon.cryptography.materialProviders.model.CreateAwsKmsDiscoveryMultiKeyringInput nativeValue) {
-    DafnySequence<? extends DafnySequence<? extends Character>> regions;
-    regions = ToDafny.RegionList(nativeValue.regions());
-    Option<DiscoveryFilter> discoveryFilter;
-    discoveryFilter = Objects.nonNull(nativeValue.discoveryFilter()) ?
-        Option.create_Some(ToDafny.DiscoveryFilter(nativeValue.discoveryFilter()))
-        : Option.create_None();
-    Option<IClientSupplier> clientSupplier;
-    clientSupplier = Objects.nonNull(nativeValue.clientSupplier()) ?
-        Option.create_Some(ToDafny.ClientSupplier(nativeValue.clientSupplier()))
-        : Option.create_None();
-    Option<DafnySequence<? extends DafnySequence<? extends Character>>> grantTokens;
-    grantTokens = Objects.nonNull(nativeValue.grantTokens()) ?
-        Option.create_Some(ToDafny.GrantTokenList(nativeValue.grantTokens()))
-        : Option.create_None();
-    return new CreateAwsKmsDiscoveryMultiKeyringInput(regions, discoveryFilter, clientSupplier, grantTokens);
-  }
-
-  public static CreateAwsKmsMrkDiscoveryMultiKeyringInput CreateAwsKmsMrkDiscoveryMultiKeyringInput(
-      software.amazon.cryptography.materialProviders.model.CreateAwsKmsMrkDiscoveryMultiKeyringInput nativeValue) {
-    DafnySequence<? extends DafnySequence<? extends Character>> regions;
-    regions = ToDafny.RegionList(nativeValue.regions());
-    Option<DiscoveryFilter> discoveryFilter;
-    discoveryFilter = Objects.nonNull(nativeValue.discoveryFilter()) ?
-        Option.create_Some(ToDafny.DiscoveryFilter(nativeValue.discoveryFilter()))
-        : Option.create_None();
-    Option<IClientSupplier> clientSupplier;
-    clientSupplier = Objects.nonNull(nativeValue.clientSupplier()) ?
-        Option.create_Some(ToDafny.ClientSupplier(nativeValue.clientSupplier()))
-        : Option.create_None();
-    Option<DafnySequence<? extends DafnySequence<? extends Character>>> grantTokens;
-    grantTokens = Objects.nonNull(nativeValue.grantTokens()) ?
-        Option.create_Some(ToDafny.GrantTokenList(nativeValue.grantTokens()))
-        : Option.create_None();
-    return new CreateAwsKmsMrkDiscoveryMultiKeyringInput(regions, discoveryFilter, clientSupplier, grantTokens);
+  public static IntermediateKeyWrapping IntermediateKeyWrapping(
+      software.amazon.cryptography.materialProviders.model.IntermediateKeyWrapping nativeValue) {
+    DerivationAlgorithm keyEncryptionKeyKdf;
+    keyEncryptionKeyKdf = ToDafny.DerivationAlgorithm(nativeValue.keyEncryptionKeyKdf());
+    DerivationAlgorithm macKeyKdf;
+    macKeyKdf = ToDafny.DerivationAlgorithm(nativeValue.macKeyKdf());
+    Encrypt pdkEncryptAlgorithm;
+    pdkEncryptAlgorithm = ToDafny.Encrypt(nativeValue.pdkEncryptAlgorithm());
+    return new IntermediateKeyWrapping(keyEncryptionKeyKdf, macKeyKdf, pdkEncryptAlgorithm);
   }
 
   public static EncryptionMaterials EncryptionMaterials(
@@ -458,41 +359,102 @@ public class ToDafny {
     return new None();
   }
 
-  public static HKDF HKDF(software.amazon.cryptography.materialProviders.model.HKDF nativeValue) {
-    DigestAlgorithm hmac;
-    hmac = software.amazon.cryptography.primitives.ToDafny.DigestAlgorithm(nativeValue.hmac());
-    Integer saltLength;
-    saltLength = (nativeValue.saltLength());
-    Integer inputKeyLength;
-    inputKeyLength = (nativeValue.inputKeyLength());
-    Integer outputKeyLength;
-    outputKeyLength = (nativeValue.outputKeyLength());
-    return new HKDF(hmac, saltLength, inputKeyLength, outputKeyLength);
+  public static DIRECT__KEY__WRAPPING DIRECT_KEY_WRAPPING(DIRECT_KEY_WRAPPING nativeValue) {
+    return new DIRECT__KEY__WRAPPING();
   }
 
-  public static DecryptMaterialsOutput DecryptMaterialsOutput(
-      software.amazon.cryptography.materialProviders.model.DecryptMaterialsOutput nativeValue) {
-    DecryptionMaterials decryptionMaterials;
-    decryptionMaterials = ToDafny.DecryptionMaterials(nativeValue.decryptionMaterials());
-    return new DecryptMaterialsOutput(decryptionMaterials);
+  public static CreateAwsKmsDiscoveryKeyringInput CreateAwsKmsDiscoveryKeyringInput(
+      software.amazon.cryptography.materialProviders.model.CreateAwsKmsDiscoveryKeyringInput nativeValue) {
+    IKeyManagementServiceClient kmsClient;
+    kmsClient = new Dafny.Com.Amazonaws.Kms.Shim(nativeValue.kmsClient(), null);
+    Option<DiscoveryFilter> discoveryFilter;
+    discoveryFilter = Objects.nonNull(nativeValue.discoveryFilter()) ?
+        Option.create_Some(ToDafny.DiscoveryFilter(nativeValue.discoveryFilter()))
+        : Option.create_None();
+    Option<DafnySequence<? extends DafnySequence<? extends Character>>> grantTokens;
+    grantTokens = Objects.nonNull(nativeValue.grantTokens()) ?
+        Option.create_Some(ToDafny.GrantTokenList(nativeValue.grantTokens()))
+        : Option.create_None();
+    return new CreateAwsKmsDiscoveryKeyringInput(kmsClient, discoveryFilter, grantTokens);
   }
 
-  public static ValidateCommitmentPolicyOnEncryptInput ValidateCommitmentPolicyOnEncryptInput(
-      software.amazon.cryptography.materialProviders.model.ValidateCommitmentPolicyOnEncryptInput nativeValue) {
-    AlgorithmSuiteId algorithm;
-    algorithm = ToDafny.AlgorithmSuiteId(nativeValue.algorithm());
+  public static MaterialProvidersConfig MaterialProvidersConfig(
+      software.amazon.cryptography.materialProviders.model.MaterialProvidersConfig nativeValue) {
+    return new MaterialProvidersConfig();
+  }
+
+  public static CreateAwsKmsMrkDiscoveryKeyringInput CreateAwsKmsMrkDiscoveryKeyringInput(
+      software.amazon.cryptography.materialProviders.model.CreateAwsKmsMrkDiscoveryKeyringInput nativeValue) {
+    IKeyManagementServiceClient kmsClient;
+    kmsClient = new Dafny.Com.Amazonaws.Kms.Shim(nativeValue.kmsClient(), null);
+    Option<DiscoveryFilter> discoveryFilter;
+    discoveryFilter = Objects.nonNull(nativeValue.discoveryFilter()) ?
+        Option.create_Some(ToDafny.DiscoveryFilter(nativeValue.discoveryFilter()))
+        : Option.create_None();
+    Option<DafnySequence<? extends DafnySequence<? extends Character>>> grantTokens;
+    grantTokens = Objects.nonNull(nativeValue.grantTokens()) ?
+        Option.create_Some(ToDafny.GrantTokenList(nativeValue.grantTokens()))
+        : Option.create_None();
+    DafnySequence<? extends Character> region;
+    region = software.amazon.dafny.conversion.ToDafny.Simple.CharacterSequence(nativeValue.region());
+    return new CreateAwsKmsMrkDiscoveryKeyringInput(kmsClient, discoveryFilter, grantTokens, region);
+  }
+
+  public static CreateAwsKmsDiscoveryMultiKeyringInput CreateAwsKmsDiscoveryMultiKeyringInput(
+      software.amazon.cryptography.materialProviders.model.CreateAwsKmsDiscoveryMultiKeyringInput nativeValue) {
+    DafnySequence<? extends DafnySequence<? extends Character>> regions;
+    regions = ToDafny.RegionList(nativeValue.regions());
+    Option<DiscoveryFilter> discoveryFilter;
+    discoveryFilter = Objects.nonNull(nativeValue.discoveryFilter()) ?
+        Option.create_Some(ToDafny.DiscoveryFilter(nativeValue.discoveryFilter()))
+        : Option.create_None();
+    Option<IClientSupplier> clientSupplier;
+    clientSupplier = Objects.nonNull(nativeValue.clientSupplier()) ?
+            Option.create_Some(ToDafny.ClientSupplier(nativeValue.clientSupplier()))
+            : Option.create_None();
+    Option<DafnySequence<? extends DafnySequence<? extends Character>>> grantTokens;
+    grantTokens = Objects.nonNull(nativeValue.grantTokens()) ?
+        Option.create_Some(ToDafny.GrantTokenList(nativeValue.grantTokens()))
+        : Option.create_None();
+    return new CreateAwsKmsDiscoveryMultiKeyringInput(regions, discoveryFilter, clientSupplier, grantTokens);
+  }
+
+  public static CreateAwsKmsMultiKeyringInput CreateAwsKmsMultiKeyringInput(
+      software.amazon.cryptography.materialProviders.model.CreateAwsKmsMultiKeyringInput nativeValue) {
+    Option<DafnySequence<? extends Character>> generator;
+    generator = Objects.nonNull(nativeValue.generator()) ?
+        Option.create_Some(software.amazon.dafny.conversion.ToDafny.Simple.CharacterSequence(nativeValue.generator()))
+        : Option.create_None();
+    Option<DafnySequence<? extends DafnySequence<? extends Character>>> kmsKeyIds;
+    kmsKeyIds = Objects.nonNull(nativeValue.kmsKeyIds()) ?
+        Option.create_Some(ToDafny.KmsKeyIdList(nativeValue.kmsKeyIds()))
+        : Option.create_None();
+    Option<IClientSupplier> clientSupplier;
+    clientSupplier = Objects.nonNull(nativeValue.clientSupplier()) ?
+            Option.create_Some(ToDafny.ClientSupplier(nativeValue.clientSupplier()))
+            : Option.create_None();
+    Option<DafnySequence<? extends DafnySequence<? extends Character>>> grantTokens;
+    grantTokens = Objects.nonNull(nativeValue.grantTokens()) ?
+        Option.create_Some(ToDafny.GrantTokenList(nativeValue.grantTokens()))
+        : Option.create_None();
+    return new CreateAwsKmsMultiKeyringInput(generator, kmsKeyIds, clientSupplier, grantTokens);
+  }
+
+  public static GetEncryptionMaterialsInput GetEncryptionMaterialsInput(
+      software.amazon.cryptography.materialProviders.model.GetEncryptionMaterialsInput nativeValue) {
+    DafnyMap<? extends DafnySequence<? extends Byte>, ? extends DafnySequence<? extends Byte>> encryptionContext;
+    encryptionContext = ToDafny.EncryptionContext(nativeValue.encryptionContext());
     CommitmentPolicy commitmentPolicy;
     commitmentPolicy = ToDafny.CommitmentPolicy(nativeValue.commitmentPolicy());
-    return new ValidateCommitmentPolicyOnEncryptInput(algorithm, commitmentPolicy);
-  }
-
-  public static DiscoveryFilter DiscoveryFilter(
-      software.amazon.cryptography.materialProviders.model.DiscoveryFilter nativeValue) {
-    DafnySequence<? extends DafnySequence<? extends Character>> accountIds;
-    accountIds = ToDafny.AccountIdList(nativeValue.accountIds());
-    DafnySequence<? extends Character> partition;
-    partition = software.amazon.dafny.conversion.ToDafny.Simple.CharacterSequence(nativeValue.partition());
-    return new DiscoveryFilter(accountIds, partition);
+    Option<AlgorithmSuiteId> algorithmSuiteId;
+    algorithmSuiteId = Objects.nonNull(nativeValue.algorithmSuiteId()) ?
+        Option.create_Some(ToDafny.AlgorithmSuiteId(nativeValue.algorithmSuiteId()))
+        : Option.create_None();
+    Option<Long> maxPlaintextLength;
+    maxPlaintextLength = Objects.nonNull(nativeValue.maxPlaintextLength()) ?
+        Option.create_Some((nativeValue.maxPlaintextLength()))
+        : Option.create_None();
+    return new GetEncryptionMaterialsInput(encryptionContext, commitmentPolicy, algorithmSuiteId, maxPlaintextLength);
   }
 
   public static InitializeEncryptionMaterialsInput InitializeEncryptionMaterialsInput(
@@ -512,30 +474,68 @@ public class ToDafny {
     return new InitializeEncryptionMaterialsInput(algorithmSuiteId, encryptionContext, signingKey, verificationKey);
   }
 
-  public static CreateAwsKmsMrkMultiKeyringInput CreateAwsKmsMrkMultiKeyringInput(
-      software.amazon.cryptography.materialProviders.model.CreateAwsKmsMrkMultiKeyringInput nativeValue) {
-    Option<DafnySequence<? extends Character>> generator;
-    generator = Objects.nonNull(nativeValue.generator()) ?
-        Option.create_Some(software.amazon.dafny.conversion.ToDafny.Simple.CharacterSequence(nativeValue.generator()))
-        : Option.create_None();
-    Option<DafnySequence<? extends DafnySequence<? extends Character>>> kmsKeyIds;
-    kmsKeyIds = Objects.nonNull(nativeValue.kmsKeyIds()) ?
-        Option.create_Some(ToDafny.KmsKeyIdList(nativeValue.kmsKeyIds()))
-        : Option.create_None();
-    Option<IClientSupplier> clientSupplier;
-    clientSupplier = Objects.nonNull(nativeValue.clientSupplier()) ?
-        Option.create_Some(ToDafny.ClientSupplier(nativeValue.clientSupplier()))
-        : Option.create_None();
-    Option<DafnySequence<? extends DafnySequence<? extends Character>>> grantTokens;
-    grantTokens = Objects.nonNull(nativeValue.grantTokens()) ?
-        Option.create_Some(ToDafny.GrantTokenList(nativeValue.grantTokens()))
-        : Option.create_None();
-    return new CreateAwsKmsMrkMultiKeyringInput(generator, kmsKeyIds, clientSupplier, grantTokens);
+  public static HKDF HKDF(software.amazon.cryptography.materialProviders.model.HKDF nativeValue) {
+    DigestAlgorithm hmac;
+    hmac = software.amazon.cryptography.primitives.ToDafny.DigestAlgorithm(nativeValue.hmac());
+    Integer saltLength;
+    saltLength = (nativeValue.saltLength());
+    Integer inputKeyLength;
+    inputKeyLength = (nativeValue.inputKeyLength());
+    Integer outputKeyLength;
+    outputKeyLength = (nativeValue.outputKeyLength());
+    return new HKDF(hmac, saltLength, inputKeyLength, outputKeyLength);
   }
 
-  public static CreateDefaultClientSupplierInput CreateDefaultClientSupplierInput(
-      software.amazon.cryptography.materialProviders.model.CreateDefaultClientSupplierInput nativeValue) {
-    return new CreateDefaultClientSupplierInput();
+  public static DecryptionMaterials DecryptionMaterials(
+      software.amazon.cryptography.materialProviders.model.DecryptionMaterials nativeValue) {
+    AlgorithmSuiteInfo algorithmSuite;
+    algorithmSuite = ToDafny.AlgorithmSuiteInfo(nativeValue.algorithmSuite());
+    DafnyMap<? extends DafnySequence<? extends Byte>, ? extends DafnySequence<? extends Byte>> encryptionContext;
+    encryptionContext = ToDafny.EncryptionContext(nativeValue.encryptionContext());
+    Option<DafnySequence<? extends Byte>> plaintextDataKey;
+    plaintextDataKey = Objects.nonNull(nativeValue.plaintextDataKey()) ?
+        Option.create_Some(software.amazon.dafny.conversion.ToDafny.Simple.ByteSequence(nativeValue.plaintextDataKey()))
+        : Option.create_None();
+    Option<DafnySequence<? extends Byte>> verificationKey;
+    verificationKey = Objects.nonNull(nativeValue.verificationKey()) ?
+        Option.create_Some(software.amazon.dafny.conversion.ToDafny.Simple.ByteSequence(nativeValue.verificationKey()))
+        : Option.create_None();
+    Option<DafnySequence<? extends Byte>> symmetricSigningKey;
+    symmetricSigningKey = Objects.nonNull(nativeValue.symmetricSigningKey()) ?
+        Option.create_Some(software.amazon.dafny.conversion.ToDafny.Simple.ByteSequence(nativeValue.symmetricSigningKey()))
+        : Option.create_None();
+    return new DecryptionMaterials(algorithmSuite, encryptionContext, plaintextDataKey, verificationKey, symmetricSigningKey);
+  }
+
+  public static OnEncryptInput OnEncryptInput(
+      software.amazon.cryptography.materialProviders.model.OnEncryptInput nativeValue) {
+    EncryptionMaterials materials;
+    materials = ToDafny.EncryptionMaterials(nativeValue.materials());
+    return new OnEncryptInput(materials);
+  }
+
+  public static ValidateCommitmentPolicyOnDecryptInput ValidateCommitmentPolicyOnDecryptInput(
+      software.amazon.cryptography.materialProviders.model.ValidateCommitmentPolicyOnDecryptInput nativeValue) {
+    AlgorithmSuiteId algorithm;
+    algorithm = ToDafny.AlgorithmSuiteId(nativeValue.algorithm());
+    CommitmentPolicy commitmentPolicy;
+    commitmentPolicy = ToDafny.CommitmentPolicy(nativeValue.commitmentPolicy());
+    return new ValidateCommitmentPolicyOnDecryptInput(algorithm, commitmentPolicy);
+  }
+
+  public static ValidEncryptionMaterialsTransitionInput ValidEncryptionMaterialsTransitionInput(
+      software.amazon.cryptography.materialProviders.model.ValidEncryptionMaterialsTransitionInput nativeValue) {
+    EncryptionMaterials start;
+    start = ToDafny.EncryptionMaterials(nativeValue.start());
+    EncryptionMaterials stop;
+    stop = ToDafny.EncryptionMaterials(nativeValue.stop());
+    return new ValidEncryptionMaterialsTransitionInput(start, stop);
+  }
+
+  public static DafnySequence<? extends Byte> GetAlgorithmSuiteInfoInput(ByteBuffer nativeValue) {
+    DafnySequence<? extends Byte> binaryId;
+    binaryId = software.amazon.dafny.conversion.ToDafny.Simple.ByteSequence(nativeValue);
+    return binaryId;
   }
 
   public static DecryptMaterialsInput DecryptMaterialsInput(
@@ -551,6 +551,26 @@ public class ToDafny {
     return new DecryptMaterialsInput(algorithmSuiteId, commitmentPolicy, encryptedDataKeys, encryptionContext);
   }
 
+  public static ValidDecryptionMaterialsTransitionInput ValidDecryptionMaterialsTransitionInput(
+      software.amazon.cryptography.materialProviders.model.ValidDecryptionMaterialsTransitionInput nativeValue) {
+    DecryptionMaterials start;
+    start = ToDafny.DecryptionMaterials(nativeValue.start());
+    DecryptionMaterials stop;
+    stop = ToDafny.DecryptionMaterials(nativeValue.stop());
+    return new ValidDecryptionMaterialsTransitionInput(start, stop);
+  }
+
+  public static CreateMultiKeyringInput CreateMultiKeyringInput(
+      software.amazon.cryptography.materialProviders.model.CreateMultiKeyringInput nativeValue) {
+    Option<IKeyring> generator;
+    generator = Objects.nonNull(nativeValue.generator()) ?
+            Option.create_Some(ToDafny.Keyring(nativeValue.generator()))
+            : Option.create_None();
+    DafnySequence<? extends IKeyring> childKeyrings;
+    childKeyrings = ToDafny.KeyringList(nativeValue.childKeyrings());
+    return new CreateMultiKeyringInput(generator, childKeyrings);
+  }
+
   public static CreateRawAesKeyringInput CreateRawAesKeyringInput(
       software.amazon.cryptography.materialProviders.model.CreateRawAesKeyringInput nativeValue) {
     DafnySequence<? extends Character> keyNamespace;
@@ -564,37 +584,116 @@ public class ToDafny {
     return new CreateRawAesKeyringInput(keyNamespace, keyName, wrappingKey, wrappingAlg);
   }
 
-  public static DafnySequence<? extends Byte> GetAlgorithmSuiteInfoInput(ByteBuffer nativeValue) {
-    DafnySequence<? extends Byte> binaryId;
-    binaryId = software.amazon.dafny.conversion.ToDafny.Simple.ByteSequence(nativeValue);
-    return binaryId;
+  public static InitializeDecryptionMaterialsInput InitializeDecryptionMaterialsInput(
+      software.amazon.cryptography.materialProviders.model.InitializeDecryptionMaterialsInput nativeValue) {
+    AlgorithmSuiteId algorithmSuiteId;
+    algorithmSuiteId = ToDafny.AlgorithmSuiteId(nativeValue.algorithmSuiteId());
+    DafnyMap<? extends DafnySequence<? extends Byte>, ? extends DafnySequence<? extends Byte>> encryptionContext;
+    encryptionContext = ToDafny.EncryptionContext(nativeValue.encryptionContext());
+    return new InitializeDecryptionMaterialsInput(algorithmSuiteId, encryptionContext);
   }
 
-  public static CreateMultiKeyringInput CreateMultiKeyringInput(
-      software.amazon.cryptography.materialProviders.model.CreateMultiKeyringInput nativeValue) {
-    Option<IKeyring> generator;
-    generator = Objects.nonNull(nativeValue.generator()) ?
-        Option.create_Some(ToDafny.Keyring(nativeValue.generator()))
+  public static EncryptedDataKey EncryptedDataKey(
+      software.amazon.cryptography.materialProviders.model.EncryptedDataKey nativeValue) {
+    DafnySequence<? extends Byte> keyProviderId;
+    keyProviderId = software.amazon.dafny.conversion.ToDafny.Simple.DafnyUtf8Bytes(nativeValue.keyProviderId());
+    DafnySequence<? extends Byte> keyProviderInfo;
+    keyProviderInfo = software.amazon.dafny.conversion.ToDafny.Simple.ByteSequence(nativeValue.keyProviderInfo());
+    DafnySequence<? extends Byte> ciphertext;
+    ciphertext = software.amazon.dafny.conversion.ToDafny.Simple.ByteSequence(nativeValue.ciphertext());
+    return new EncryptedDataKey(keyProviderId, keyProviderInfo, ciphertext);
+  }
+
+  public static OnEncryptOutput OnEncryptOutput(
+      software.amazon.cryptography.materialProviders.model.OnEncryptOutput nativeValue) {
+    EncryptionMaterials materials;
+    materials = ToDafny.EncryptionMaterials(nativeValue.materials());
+    return new OnEncryptOutput(materials);
+  }
+
+  public static CreateAwsKmsRsaKeyringInput CreateAwsKmsRsaKeyringInput(
+          software.amazon.cryptography.materialProviders.model.CreateAwsKmsRsaKeyringInput nativeValue) {
+    Option<DafnySequence<? extends Byte>> publicKey;
+    publicKey = Objects.nonNull(nativeValue.publicKey()) ?
+            Option.create_Some(software.amazon.dafny.conversion.ToDafny.Simple.ByteSequence(nativeValue.publicKey()))
+            : Option.create_None();
+    DafnySequence<? extends Character> kmsKeyId;
+    kmsKeyId = software.amazon.dafny.conversion.ToDafny.Simple.CharacterSequence(nativeValue.kmsKeyId());
+    EncryptionAlgorithmSpec encryptionAlgorithm;
+    encryptionAlgorithm = Dafny.Com.Amazonaws.Kms.ToDafny.EncryptionAlgorithmSpec(nativeValue.encryptionAlgorithm());
+    Option<IKeyManagementServiceClient> kmsClient;
+    kmsClient = Objects.nonNull(nativeValue.kmsClient()) ?
+            Option.create_Some((new Dafny.Com.Amazonaws.Kms.Shim(nativeValue.kmsClient(), null)))
+            : Option.create_None();
+    Option<DafnySequence<? extends DafnySequence<? extends Character>>> grantTokens;
+    grantTokens = Objects.nonNull(nativeValue.grantTokens()) ?
+            Option.create_Some(ToDafny.GrantTokenList(nativeValue.grantTokens()))
+            : Option.create_None();
+    return new CreateAwsKmsRsaKeyringInput(publicKey, kmsKeyId, encryptionAlgorithm, kmsClient, grantTokens);
+  }
+
+  public static CreateAwsKmsMrkKeyringInput CreateAwsKmsMrkKeyringInput(
+      software.amazon.cryptography.materialProviders.model.CreateAwsKmsMrkKeyringInput nativeValue) {
+    DafnySequence<? extends Character> kmsKeyId;
+    kmsKeyId = software.amazon.dafny.conversion.ToDafny.Simple.CharacterSequence(nativeValue.kmsKeyId());
+    IKeyManagementServiceClient kmsClient;
+    kmsClient = new Dafny.Com.Amazonaws.Kms.Shim(nativeValue.kmsClient(), null);
+    Option<DafnySequence<? extends DafnySequence<? extends Character>>> grantTokens;
+    grantTokens = Objects.nonNull(nativeValue.grantTokens()) ?
+        Option.create_Some(ToDafny.GrantTokenList(nativeValue.grantTokens()))
         : Option.create_None();
-    DafnySequence<? extends IKeyring> childKeyrings;
-    childKeyrings = ToDafny.KeyringList(nativeValue.childKeyrings());
-    return new CreateMultiKeyringInput(generator, childKeyrings);
+    return new CreateAwsKmsMrkKeyringInput(kmsKeyId, kmsClient, grantTokens);
   }
 
-  public static ECDSA ECDSA(
-      software.amazon.cryptography.materialProviders.model.ECDSA nativeValue) {
-    ECDSASignatureAlgorithm curve;
-    curve = software.amazon.cryptography.primitives.ToDafny.ECDSASignatureAlgorithm(nativeValue.curve());
-    return new ECDSA(curve);
+  public static CreateAwsKmsHierarchicalKeyringInput CreateAwsKmsHierarchicalKeyringInput(
+      software.amazon.cryptography.materialProviders.model.CreateAwsKmsHierarchicalKeyringInput nativeValue) {
+    DafnySequence<? extends Character> branchKeyId;
+    branchKeyId = software.amazon.dafny.conversion.ToDafny.Simple.CharacterSequence(nativeValue.branchKeyId());
+    DafnySequence<? extends Character> kmsKeyId;
+    kmsKeyId = software.amazon.dafny.conversion.ToDafny.Simple.CharacterSequence(nativeValue.kmsKeyId());
+    IKeyManagementServiceClient kmsClient;
+    kmsClient = new Dafny.Com.Amazonaws.Kms.Shim(nativeValue.kmsClient(), null);
+    IDynamoDB__20120810Client ddbClient;
+    ddbClient = new Dafny.Com.Amazonaws.Dynamodb.Shim(nativeValue.ddbClient(), null);
+    DafnySequence<? extends Character> branchKeyStoreArn;
+    branchKeyStoreArn = software.amazon.dafny.conversion.ToDafny.Simple.CharacterSequence(nativeValue.branchKeyStoreArn());
+    Long ttlSeconds;
+    ttlSeconds = (nativeValue.ttlSeconds());
+    Option<Integer> maxCacheSize;
+    maxCacheSize = Objects.nonNull(nativeValue.maxCacheSize()) ?
+        Option.create_Some((nativeValue.maxCacheSize()))
+        : Option.create_None();
+    Option<DafnySequence<? extends DafnySequence<? extends Character>>> grantTokens;
+    grantTokens = Objects.nonNull(nativeValue.grantTokens()) ?
+        Option.create_Some(ToDafny.GrantTokenList(nativeValue.grantTokens()))
+        : Option.create_None();
+    return new CreateAwsKmsHierarchicalKeyringInput(branchKeyId, kmsKeyId, kmsClient, ddbClient, branchKeyStoreArn, ttlSeconds, maxCacheSize, grantTokens);
   }
 
-  public static ValidDecryptionMaterialsTransitionInput ValidDecryptionMaterialsTransitionInput(
-      software.amazon.cryptography.materialProviders.model.ValidDecryptionMaterialsTransitionInput nativeValue) {
-    DecryptionMaterials start;
-    start = ToDafny.DecryptionMaterials(nativeValue.start());
-    DecryptionMaterials stop;
-    stop = ToDafny.DecryptionMaterials(nativeValue.stop());
-    return new ValidDecryptionMaterialsTransitionInput(start, stop);
+  public static GetEncryptionMaterialsOutput GetEncryptionMaterialsOutput(
+      software.amazon.cryptography.materialProviders.model.GetEncryptionMaterialsOutput nativeValue) {
+    EncryptionMaterials encryptionMaterials;
+    encryptionMaterials = ToDafny.EncryptionMaterials(nativeValue.encryptionMaterials());
+    return new GetEncryptionMaterialsOutput(encryptionMaterials);
+  }
+
+  public static OnDecryptOutput OnDecryptOutput(
+      software.amazon.cryptography.materialProviders.model.OnDecryptOutput nativeValue) {
+    DecryptionMaterials materials;
+    materials = ToDafny.DecryptionMaterials(nativeValue.materials());
+    return new OnDecryptOutput(materials);
+  }
+
+  public static Error Error(InvalidDecryptionMaterialsTransition nativeValue) {
+    DafnySequence<? extends Character> message;
+    message = software.amazon.dafny.conversion.ToDafny.Simple.CharacterSequence(nativeValue.message());
+    return new Error_InvalidDecryptionMaterialsTransition(message);
+  }
+
+  public static Error Error(InvalidAlgorithmSuiteInfoOnDecrypt nativeValue) {
+    DafnySequence<? extends Character> message;
+    message = software.amazon.dafny.conversion.ToDafny.Simple.CharacterSequence(nativeValue.message());
+    return new Error_InvalidAlgorithmSuiteInfoOnDecrypt(message);
   }
 
   public static Error Error(InvalidDecryptionMaterials nativeValue) {
@@ -609,6 +708,18 @@ public class ToDafny {
     return new Error_InvalidAlgorithmSuiteInfo(message);
   }
 
+  public static Error Error(AwsCryptographicMaterialProvidersException nativeValue) {
+    DafnySequence<? extends Character> message;
+    message = software.amazon.dafny.conversion.ToDafny.Simple.CharacterSequence(nativeValue.message());
+    return new Error_AwsCryptographicMaterialProvidersException(message);
+  }
+
+  public static Error Error(InvalidEncryptionMaterialsTransition nativeValue) {
+    DafnySequence<? extends Character> message;
+    message = software.amazon.dafny.conversion.ToDafny.Simple.CharacterSequence(nativeValue.message());
+    return new Error_InvalidEncryptionMaterialsTransition(message);
+  }
+
   public static Error Error(InvalidAlgorithmSuiteInfoOnEncrypt nativeValue) {
     DafnySequence<? extends Character> message;
     message = software.amazon.dafny.conversion.ToDafny.Simple.CharacterSequence(nativeValue.message());
@@ -619,66 +730,6 @@ public class ToDafny {
     DafnySequence<? extends Character> message;
     message = software.amazon.dafny.conversion.ToDafny.Simple.CharacterSequence(nativeValue.message());
     return new Error_InvalidEncryptionMaterials(message);
-  }
-
-  public static Error Error(InvalidDecryptionMaterialsTransition nativeValue) {
-    DafnySequence<? extends Character> message;
-    message = software.amazon.dafny.conversion.ToDafny.Simple.CharacterSequence(nativeValue.message());
-    return new Error_InvalidDecryptionMaterialsTransition(message);
-  }
-
-  public static Error Error(InvalidEncryptionMaterialsTransition nativeValue) {
-    DafnySequence<? extends Character> message;
-    message = software.amazon.dafny.conversion.ToDafny.Simple.CharacterSequence(nativeValue.message());
-    return new Error_InvalidEncryptionMaterialsTransition(message);
-  }
-
-  public static Error Error(InvalidAlgorithmSuiteInfoOnDecrypt nativeValue) {
-    DafnySequence<? extends Character> message;
-    message = software.amazon.dafny.conversion.ToDafny.Simple.CharacterSequence(nativeValue.message());
-    return new Error_InvalidAlgorithmSuiteInfoOnDecrypt(message);
-  }
-
-  public static Error Error(AwsCryptographicMaterialProvidersException nativeValue) {
-    DafnySequence<? extends Character> message;
-    message = software.amazon.dafny.conversion.ToDafny.Simple.CharacterSequence(nativeValue.message());
-    return new Error_AwsCryptographicMaterialProvidersException(message);
-  }
-
-  public static AesWrappingAlg AesWrappingAlg(
-      software.amazon.cryptography.materialProviders.model.AesWrappingAlg nativeValue) {
-    switch (nativeValue) {
-      case ALG_AES128_GCM_IV12_TAG16: {
-        return AesWrappingAlg.create_ALG__AES128__GCM__IV12__TAG16();
-      }
-      case ALG_AES192_GCM_IV12_TAG16: {
-        return AesWrappingAlg.create_ALG__AES192__GCM__IV12__TAG16();
-      }
-      case ALG_AES256_GCM_IV12_TAG16: {
-        return AesWrappingAlg.create_ALG__AES256__GCM__IV12__TAG16();
-      }
-      default: {
-        throw new RuntimeException("Cannot convert " + nativeValue + " to Dafny.Aws.Cryptography.MaterialProviders.Types.AesWrappingAlg.");
-      }
-    }
-  }
-
-  public static ESDKCommitmentPolicy ESDKCommitmentPolicy(
-      software.amazon.cryptography.materialProviders.model.ESDKCommitmentPolicy nativeValue) {
-    switch (nativeValue) {
-      case FORBID_ENCRYPT_ALLOW_DECRYPT: {
-        return ESDKCommitmentPolicy.create_FORBID__ENCRYPT__ALLOW__DECRYPT();
-      }
-      case REQUIRE_ENCRYPT_ALLOW_DECRYPT: {
-        return ESDKCommitmentPolicy.create_REQUIRE__ENCRYPT__ALLOW__DECRYPT();
-      }
-      case REQUIRE_ENCRYPT_REQUIRE_DECRYPT: {
-        return ESDKCommitmentPolicy.create_REQUIRE__ENCRYPT__REQUIRE__DECRYPT();
-      }
-      default: {
-        throw new RuntimeException("Cannot convert " + nativeValue + " to Dafny.Aws.Cryptography.MaterialProviders.Types.ESDKCommitmentPolicy.");
-      }
-    }
   }
 
   public static ESDKAlgorithmSuiteId ESDKAlgorithmSuiteId(
@@ -747,31 +798,72 @@ public class ToDafny {
     }
   }
 
-  public static SignatureAlgorithm SignatureAlgorithm(
-      software.amazon.cryptography.materialProviders.model.SignatureAlgorithm nativeValue) {
-    if (Objects.nonNull(nativeValue.ECDSA())) {
-      return SignatureAlgorithm.create_ECDSA(ToDafny.ECDSA(nativeValue.ECDSA()));
+  public static ESDKCommitmentPolicy ESDKCommitmentPolicy(
+      software.amazon.cryptography.materialProviders.model.ESDKCommitmentPolicy nativeValue) {
+    switch (nativeValue) {
+      case FORBID_ENCRYPT_ALLOW_DECRYPT: {
+        return ESDKCommitmentPolicy.create_FORBID__ENCRYPT__ALLOW__DECRYPT();
+      }
+      case REQUIRE_ENCRYPT_ALLOW_DECRYPT: {
+        return ESDKCommitmentPolicy.create_REQUIRE__ENCRYPT__ALLOW__DECRYPT();
+      }
+      case REQUIRE_ENCRYPT_REQUIRE_DECRYPT: {
+        return ESDKCommitmentPolicy.create_REQUIRE__ENCRYPT__REQUIRE__DECRYPT();
+      }
+      default: {
+        throw new RuntimeException("Cannot convert " + nativeValue + " to Dafny.Aws.Cryptography.MaterialProviders.Types.ESDKCommitmentPolicy.");
+      }
     }
-    if (Objects.nonNull(nativeValue.None())) {
-      return SignatureAlgorithm.create_None(ToDafny.None(nativeValue.None()));
+  }
+
+  public static DBEAlgorithmSuiteId DBEAlgorithmSuiteId(
+      software.amazon.cryptography.materialProviders.model.DBEAlgorithmSuiteId nativeValue) {
+    switch (nativeValue) {
+      case ALG_AES_256_GCM_HKDF_SHA512_COMMIT_KEY_SYMSIG_HMAC_SHA384: {
+        return DBEAlgorithmSuiteId.create_ALG__AES__256__GCM__HKDF__SHA512__COMMIT__KEY__SYMSIG__HMAC__SHA384();
+      }
+      case ALG_AES_256_GCM_HKDF_SHA512_COMMIT_KEY_ECDSA_P384_SYMSIG_HMAC_SHA384: {
+        return DBEAlgorithmSuiteId.create_ALG__AES__256__GCM__HKDF__SHA512__COMMIT__KEY__ECDSA__P384__SYMSIG__HMAC__SHA384();
+      }
+      default: {
+        throw new RuntimeException("Cannot convert " + nativeValue + " to Dafny.Aws.Cryptography.MaterialProviders.Types.DBEAlgorithmSuiteId.");
+      }
     }
-    throw new IllegalArgumentException("Cannot convert " + nativeValue + " to Dafny.Aws.Cryptography.MaterialProviders.Types.SignatureAlgorithm.");
+  }
+
+  public static AesWrappingAlg AesWrappingAlg(
+      software.amazon.cryptography.materialProviders.model.AesWrappingAlg nativeValue) {
+    switch (nativeValue) {
+      case ALG_AES128_GCM_IV12_TAG16: {
+        return AesWrappingAlg.create_ALG__AES128__GCM__IV12__TAG16();
+      }
+      case ALG_AES192_GCM_IV12_TAG16: {
+        return AesWrappingAlg.create_ALG__AES192__GCM__IV12__TAG16();
+      }
+      case ALG_AES256_GCM_IV12_TAG16: {
+        return AesWrappingAlg.create_ALG__AES256__GCM__IV12__TAG16();
+      }
+      default: {
+        throw new RuntimeException("Cannot convert " + nativeValue + " to Dafny.Aws.Cryptography.MaterialProviders.Types.AesWrappingAlg.");
+      }
+    }
+  }
+
+  public static DBECommitmentPolicy DBECommitmentPolicy(
+          software.amazon.cryptography.materialProviders.model.DBECommitmentPolicy nativeValue) {
+    switch (nativeValue) {
+      case REQUIRE_ENCRYPT_REQUIRE_DECRYPT: {
+        return DBECommitmentPolicy.create(); // TODO Dafny converts datatypes with a single constructor in a different way than expected
+      }
+      default: {
+        throw new RuntimeException("Cannot convert " + nativeValue + " to Dafny.Aws.Cryptography.MaterialProviders.Types.DBECommitmentPolicy.");
+      }
+    }
   }
 
   public static Encrypt Encrypt(
       software.amazon.cryptography.materialProviders.model.Encrypt nativeValue) {
     return Encrypt.create(software.amazon.cryptography.primitives.ToDafny.AES_GCM(nativeValue.AES_GCM()));
-  }
-
-  public static AlgorithmSuiteId AlgorithmSuiteId(
-      software.amazon.cryptography.materialProviders.model.AlgorithmSuiteId nativeValue) {
-    if (Objects.nonNull(nativeValue.ESDK())) {
-      return AlgorithmSuiteId.create_ESDK(ToDafny.ESDKAlgorithmSuiteId(nativeValue.ESDK()));
-    }
-    if (Objects.nonNull(nativeValue.DBE())) {
-      return AlgorithmSuiteId.create_DBE(ToDafny.DBEAlgorithmSuiteId(nativeValue.DBE()));
-    }
-    throw new IllegalArgumentException("Cannot convert " + nativeValue + " to Dafny.Aws.Cryptography.MaterialProviders.Types.AlgorithmSuiteId.");
   }
 
   public static DerivationAlgorithm DerivationAlgorithm(
@@ -788,6 +880,28 @@ public class ToDafny {
     throw new IllegalArgumentException("Cannot convert " + nativeValue + " to Dafny.Aws.Cryptography.MaterialProviders.Types.DerivationAlgorithm.");
   }
 
+  public static AlgorithmSuiteId AlgorithmSuiteId(
+      software.amazon.cryptography.materialProviders.model.AlgorithmSuiteId nativeValue) {
+    if (Objects.nonNull(nativeValue.ESDK())) {
+      return AlgorithmSuiteId.create_ESDK(ToDafny.ESDKAlgorithmSuiteId(nativeValue.ESDK()));
+    }
+    if (Objects.nonNull(nativeValue.DBE())) {
+      return AlgorithmSuiteId.create_DBE(ToDafny.DBEAlgorithmSuiteId(nativeValue.DBE()));
+    }
+    throw new IllegalArgumentException("Cannot convert " + nativeValue + " to Dafny.Aws.Cryptography.MaterialProviders.Types.AlgorithmSuiteId.");
+  }
+
+  public static SymmetricSignatureAlgorithm SymmetricSignatureAlgorithm(
+      software.amazon.cryptography.materialProviders.model.SymmetricSignatureAlgorithm nativeValue) {
+    if (Objects.nonNull(nativeValue.HMAC())) {
+      return SymmetricSignatureAlgorithm.create_HMAC(software.amazon.cryptography.primitives.ToDafny.DigestAlgorithm(nativeValue.HMAC()));
+    }
+    if (Objects.nonNull(nativeValue.None())) {
+      return SymmetricSignatureAlgorithm.create_None(ToDafny.None(nativeValue.None()));
+    }
+    throw new IllegalArgumentException("Cannot convert " + nativeValue + " to Dafny.Aws.Cryptography.MaterialProviders.Types.SymmetricSignatureAlgorithm.");
+  }
+
   public static CommitmentPolicy CommitmentPolicy(
       software.amazon.cryptography.materialProviders.model.CommitmentPolicy nativeValue) {
     if (Objects.nonNull(nativeValue.ESDK())) {
@@ -799,12 +913,34 @@ public class ToDafny {
     throw new IllegalArgumentException("Cannot convert " + nativeValue + " to Dafny.Aws.Cryptography.MaterialProviders.Types.CommitmentPolicy.");
   }
 
-  public static DafnySequence<? extends DafnySequence<? extends Character>> AccountIdList(
-      List<String> nativeValue) {
+  public static EdkWrappingAlgorithm EdkWrappingAlgorithm(
+      software.amazon.cryptography.materialProviders.model.EdkWrappingAlgorithm nativeValue) {
+    if (Objects.nonNull(nativeValue.DIRECT_KEY_WRAPPING())) {
+      return EdkWrappingAlgorithm.create_DIRECT__KEY__WRAPPING(ToDafny.DIRECT_KEY_WRAPPING(nativeValue.DIRECT_KEY_WRAPPING()));
+    }
+    if (Objects.nonNull(nativeValue.IntermediateKeyWrapping())) {
+      return EdkWrappingAlgorithm.create_IntermediateKeyWrapping(ToDafny.IntermediateKeyWrapping(nativeValue.IntermediateKeyWrapping()));
+    }
+    throw new IllegalArgumentException("Cannot convert " + nativeValue + " to Dafny.Aws.Cryptography.MaterialProviders.Types.EdkWrappingAlgorithm.");
+  }
+
+  public static SignatureAlgorithm SignatureAlgorithm(
+      software.amazon.cryptography.materialProviders.model.SignatureAlgorithm nativeValue) {
+    if (Objects.nonNull(nativeValue.ECDSA())) {
+      return SignatureAlgorithm.create_ECDSA(ToDafny.ECDSA(nativeValue.ECDSA()));
+    }
+    if (Objects.nonNull(nativeValue.None())) {
+      return SignatureAlgorithm.create_None(ToDafny.None(nativeValue.None()));
+    }
+    throw new IllegalArgumentException("Cannot convert " + nativeValue + " to Dafny.Aws.Cryptography.MaterialProviders.Types.SignatureAlgorithm.");
+  }
+
+  public static DafnySequence<? extends DafnySequence<? extends Byte>> SymmetricSigningKeyList(
+      List<ByteBuffer> nativeValue) {
     return software.amazon.dafny.conversion.ToDafny.Aggregate.GenericToSequence(
         nativeValue, 
-        software.amazon.dafny.conversion.ToDafny.Simple::CharacterSequence, 
-        DafnySequence._typeDescriptor(TypeDescriptor.CHAR));
+        software.amazon.dafny.conversion.ToDafny.Simple::ByteSequence, 
+        DafnySequence._typeDescriptor(TypeDescriptor.BYTE));
   }
 
   public static DafnySequence<? extends DafnySequence<? extends Character>> GrantTokenList(
@@ -813,6 +949,31 @@ public class ToDafny {
         nativeValue, 
         software.amazon.dafny.conversion.ToDafny.Simple::CharacterSequence, 
         DafnySequence._typeDescriptor(TypeDescriptor.CHAR));
+  }
+
+  public static DafnySequence<? extends DafnySequence<? extends Character>> AccountIdList(
+      List<String> nativeValue) {
+    return software.amazon.dafny.conversion.ToDafny.Aggregate.GenericToSequence(
+        nativeValue, 
+        software.amazon.dafny.conversion.ToDafny.Simple::CharacterSequence, 
+        DafnySequence._typeDescriptor(TypeDescriptor.CHAR));
+  }
+
+  public static DafnySequence<? extends DafnySequence<? extends Character>> RegionList(
+      List<String> nativeValue) {
+    return software.amazon.dafny.conversion.ToDafny.Aggregate.GenericToSequence(
+        nativeValue, 
+        software.amazon.dafny.conversion.ToDafny.Simple::CharacterSequence, 
+        DafnySequence._typeDescriptor(TypeDescriptor.CHAR));
+  }
+
+  public static <I extends software.amazon.cryptography.materialProviders.IKeyring> DafnySequence<? extends IKeyring> KeyringList(
+          List<I> nativeValue
+  ) {
+    return software.amazon.dafny.conversion.ToDafny.Aggregate.GenericToSequence(
+            nativeValue,
+            software.amazon.cryptography.materialProviders.ToDafny::Keyring,
+            TypeDescriptor.reference(IKeyring.class));
   }
 
   public static DafnySequence<? extends DafnySequence<? extends Character>> KmsKeyIdList(
@@ -829,23 +990,6 @@ public class ToDafny {
         nativeValue, 
         software.amazon.cryptography.materialProviders.ToDafny::EncryptedDataKey, 
         EncryptedDataKey._typeDescriptor());
-  }
-
-   public static <I extends software.amazon.cryptography.materialProviders.IKeyring> DafnySequence<? extends IKeyring> KeyringList(
-          List<I> nativeValue
-  ) {
-    return software.amazon.dafny.conversion.ToDafny.Aggregate.GenericToSequence(
-        nativeValue, 
-        software.amazon.cryptography.materialProviders.ToDafny::Keyring, 
-        TypeDescriptor.reference(IKeyring.class));
-  }
-
-  public static DafnySequence<? extends DafnySequence<? extends Character>> RegionList(
-      List<String> nativeValue) {
-    return software.amazon.dafny.conversion.ToDafny.Aggregate.GenericToSequence(
-        nativeValue, 
-        software.amazon.dafny.conversion.ToDafny.Simple::CharacterSequence, 
-        DafnySequence._typeDescriptor(TypeDescriptor.CHAR));
   }
 
   public static DafnyMap<? extends DafnySequence<? extends Byte>, ? extends DafnySequence<? extends Byte>> EncryptionContext(
@@ -872,77 +1016,5 @@ public class ToDafny {
           software.amazon.cryptography.materialProviders.IClientSupplier nativeValue
   ) {
     return ClientSupplier.create(nativeValue).impl();
-  }
-
-    public static SymmetricSignatureAlgorithm SymmetricSignatureAlgorithm(
-      software.amazon.cryptography.materialProviders.model.SymmetricSignatureAlgorithm nativeValue) {
-    if (Objects.nonNull(nativeValue.HMAC())) {
-      return SymmetricSignatureAlgorithm.create_HMAC(software.amazon.cryptography.primitives.ToDafny.DigestAlgorithm(nativeValue.HMAC()));
-    }
-    if (Objects.nonNull(nativeValue.None())) {
-      return SymmetricSignatureAlgorithm.create_None(ToDafny.None(nativeValue.None()));
-    }
-    throw new IllegalArgumentException("Cannot convert " + nativeValue + " to Dafny.Aws.Cryptography.MaterialProviders.Types.SymmetricSignatureAlgorithm.");
-  }
-
-  public static EdkWrappingAlgorithm EdkWrappingAlgorithm(
-      software.amazon.cryptography.materialProviders.model.EdkWrappingAlgorithm nativeValue) {
-    if (Objects.nonNull(nativeValue.DIRECT_KEY_WRAPPING())) {
-      return EdkWrappingAlgorithm.create_DIRECT__KEY__WRAPPING(ToDafny.DIRECT_KEY_WRAPPING(nativeValue.DIRECT_KEY_WRAPPING()));
-    }
-    if (Objects.nonNull(nativeValue.IntermediateKeyWrapping())) {
-      return EdkWrappingAlgorithm.create_IntermediateKeyWrapping(ToDafny.IntermediateKeyWrapping(nativeValue.IntermediateKeyWrapping()));
-    }
-    throw new IllegalArgumentException("Cannot convert " + nativeValue + " to Dafny.Aws.Cryptography.MaterialProviders.Types.EdkWrappingAlgorithm.");
-  }
-
-  public static DIRECT__KEY__WRAPPING DIRECT_KEY_WRAPPING(DIRECT_KEY_WRAPPING nativeValue) {
-    return new DIRECT__KEY__WRAPPING();
-  }
-
-  public static DBEAlgorithmSuiteId DBEAlgorithmSuiteId(
-      software.amazon.cryptography.materialProviders.model.DBEAlgorithmSuiteId nativeValue) {
-    switch (nativeValue) {
-      case ALG_AES_256_GCM_HKDF_SHA512_COMMIT_KEY_SYMSIG_HMAC_SHA384: {
-        return DBEAlgorithmSuiteId.create_ALG__AES__256__GCM__HKDF__SHA512__COMMIT__KEY__SYMSIG__HMAC__SHA384();
-      }
-      case ALG_AES_256_GCM_HKDF_SHA512_COMMIT_KEY_ECDSA_P384_SYMSIG_HMAC_SHA384: {
-        return DBEAlgorithmSuiteId.create_ALG__AES__256__GCM__HKDF__SHA512__COMMIT__KEY__ECDSA__P384__SYMSIG__HMAC__SHA384();
-      }
-      default: {
-        throw new RuntimeException("Cannot convert " + nativeValue + " to Dafny.Aws.Cryptography.MaterialProviders.Types.DBEAlgorithmSuiteId.");
-      }
-    }
-  }
-
-  public static IntermediateKeyWrapping IntermediateKeyWrapping(
-      software.amazon.cryptography.materialProviders.model.IntermediateKeyWrapping nativeValue) {
-    DerivationAlgorithm keyEncryptionKeyKdf;
-    keyEncryptionKeyKdf = ToDafny.DerivationAlgorithm(nativeValue.keyEncryptionKeyKdf());
-    DerivationAlgorithm macKeyKdf;
-    macKeyKdf = ToDafny.DerivationAlgorithm(nativeValue.macKeyKdf());
-    Encrypt pdkEncryptAlgorithm;
-    pdkEncryptAlgorithm = ToDafny.Encrypt(nativeValue.pdkEncryptAlgorithm());
-    return new IntermediateKeyWrapping(keyEncryptionKeyKdf, macKeyKdf, pdkEncryptAlgorithm);
-  }
-
-  public static DBECommitmentPolicy DBECommitmentPolicy(
-      software.amazon.cryptography.materialProviders.model.DBECommitmentPolicy nativeValue) {
-    switch (nativeValue) {
-      case REQUIRE_ENCRYPT_REQUIRE_DECRYPT: {
-        return DBECommitmentPolicy.create(); // TODO Dafny converts datatypes with a single constructor in a different way than expected
-      }
-      default: {
-        throw new RuntimeException("Cannot convert " + nativeValue + " to Dafny.Aws.Cryptography.MaterialProviders.Types.DBECommitmentPolicy.");
-      }
-    }
-  }
-
-  public static DafnySequence<? extends DafnySequence<? extends Byte>> SymmetricSigningKeyList(
-      List<ByteBuffer> nativeValue) {
-    return software.amazon.dafny.conversion.ToDafny.Aggregate.GenericToSequence(
-        nativeValue, 
-        software.amazon.dafny.conversion.ToDafny.Simple::ByteSequence, 
-        DafnySequence._typeDescriptor(TypeDescriptor.BYTE));
   }
 }
