AwsCryptographicMaterialProviders/src/Keyrings/AwsKms/AwsKmsHierarchicalKeyring.dfy
@@ -35,38 +35,60 @@ module AwsKmsHierarchicalKeyring {
   import HKDF
   import HMAC
   import opened AESEncryption
+  import Aws.Cryptography.Primitives
   
-  // UTF-8 encoded "TRUSS_KEYWRAP_ENC"
-  const TRUSS_KEYWRAP_ENC: UTF8.ValidUTF8Bytes :=
-    var s := [0x54, 0x52, 0x55, 0x53, 0x53, 0x5f, 0x4b, 0x45, 0x59, 0x57, 0x52, 0x41, 0x50, 0x5f, 0x45, 0x4e, 0x43];
-    assert UTF8.ValidUTF8Range(s, 0, 17);
-    s
+  const BRANCH_KEY_STORE_GSI := "Active-Keys";
+  const BRANCH_KEY_FIELD := "enc";
+  const VERSION_FIELD := "version";
+  const BRANCH_KEY_IDENTIFIER_FIELD := "branch-key-id";
   
-  // UTF-8 encoded "TRUSS_KEYWRAP_MAC"
-  const TRUSS_KEYWRAP_MAC: UTF8.ValidUTF8Bytes :=
-    var s := [0x54, 0x52, 0x55, 0x53, 0x53, 0x5f, 0x4b, 0x45, 0x59, 0x57, 0x52, 0x41, 0x50, 0x5f, 0x4d, 0x41, 0x43];
-    assert UTF8.ValidUTF8Range(s, 0, 17);
-    s
+  const KEY_CONDITION_EXPRESSION := "#status = :status and #branch_key_id = :branch_key_id";
+  const EXPRESSION_ATTRIBUTE_NAMES := map[
+    "#status"       := "status",
+    "#branch_key_id" := "branch-key-id"
+  ];
+  const EXPRESSION_ATTRIBUTE_VALUE_STATUS_KEY := ":status";
+  const EXPRESSION_ATTRIBUTE_VALUE_STATUS_VALUE := "ACTIVE";
+  const EXPRESSION_ATTRIBUTE_VALUE_BRANCH_KEY := ":branch_key_id";
+  
+  const H_WRAP_SALT_LEN: Types.PositiveInteger := 16;
+  const H_WRAP_NONCE_LEN: Types.PositiveInteger := 12;
+  const DERIVED_BRANCH_KEY_EXPECTED_LENGTH: Types.PositiveInteger := 32;
+  const AES_256_ENC_KEY_LENGTH: int32 := 32;
+  const AES_256_ENC_TAG_LENGTH: int32 := 16;
+  const AES_256_ENC_IV_LENGTH: int32 := 12;
+  const AES_256_ENC_ALG := Crypto.AES_GCM(
+    keyLength := AES_256_ENC_KEY_LENGTH,
+    //= aws-encryption-sdk-specification/framework/aws-kms/aws-kms-hierarchical-keyring.md#branch-key-wrapping
+    //= type=implication
+    //# MUST use an authentication tag byte of length 16.
+    tagLength := AES_256_ENC_TAG_LENGTH,
+    ivLength := AES_256_ENC_IV_LENGTH
+  );
 
-  // UTF-8 encoded "ACTIVE"
-  const ACTIVE: UTF8.ValidUTF8Bytes :=
-    var s := [0x41,  0x43,  0x54,  0x49,  0x56,  0x45];
-    assert UTF8.ValidUTF8Range(s, 0, 6);
-    s
+  const EXPECTED_EDK_CIPHERTEXT_LENGTH := 112;
+  const EDK_CIPHERTEXT_VERSION_LENGTH: int32 := 36;
+  const EDK_CIPHERTEXT_BRANCH_KEY_VERSION_INDEX := H_WRAP_SALT_LEN + H_WRAP_NONCE_LEN; 
+  const EDK_CIPHERTEXT_VERSION_INDEX := EDK_CIPHERTEXT_BRANCH_KEY_VERSION_INDEX + EDK_CIPHERTEXT_VERSION_LENGTH;
+  const EDK_CIPHERTEXT_KEY_INDEX := EDK_CIPHERTEXT_VERSION_INDEX + AES_256_ENC_KEY_LENGTH;
 
   
-  type branchKeyRecordMap = m: map<DDB.AttributeName, DDB.AttributeValue> | branchKeyRecordMap?(m) witness *
-  predicate branchKeyRecordMap?(m: map<DDB.AttributeName, DDB.AttributeValue>) {
-    "amzn-ddbec-metadata" in m && "amzn-ddbec-enc" in m && "keyNamespace" in m 
-      && "Version" in m && "Status" in m
+  type branchKeyItem = m: DDB.AttributeMap | branchKeyItemHasRequiredAttributes?(m) witness *
+  predicate method branchKeyItemHasRequiredAttributes?(m: DDB.AttributeMap) {
+    && "branch-key-id" in m && m["branch-key-id"].S?
+    && "version" in m && m["version"].S?
+    && "status" in m && m["status"].S?
+    && "create-time" in m && m["create-time"].S?
+    && "hierarchy-version" in m && m["hierarchy-version"].N?
+    && BRANCH_KEY_FIELD in m && m[BRANCH_KEY_FIELD].B?
+    && KMS.IsValid_CiphertextType(m[BRANCH_KEY_FIELD].B)
+    && var tmpM := m - {BRANCH_KEY_FIELD};
+    && forall k | k in tmpM :: ValueToString(tmpM[k]).Success?
   }
-  
-  type branchKeyRecordEncContextMap = m: map<DDB.AttributeName, DDB.AttributeValue> | branchKeyRecordEncContextMap?(m) witness *
-  predicate branchKeyRecordEncContextMap?(m: map<DDB.AttributeName, DDB.AttributeValue>) {
-    "Partition Key" in m && "Region" in m && "Sort Key" in m && "TableName" in m
-  }
 
-
+  //= aws-encryption-sdk-specification/framework/aws-kms/aws-kms-hierarchical-keyring.md#interface
+  //= type=implication
+  //# MUST implement the [AWS Encryption SDK Keyring interface](../keyring-interface.md#interface)
   class AwsKmsHierarchicalKeyring
     extends Keyring.VerifiableInterface
   {
@@ -75,10 +97,12 @@ module AwsKmsHierarchicalKeyring {
     const branchKeyId: string
     const awsKmsKey: AwsKmsIdentifierString
     const awsKmsArn: AwsKmsIdentifier
-    const branchKeysTableName: string
-    const ttlMilliseconds: int64
-    const maxCacheSize: int32
+    const branchKeyStoreArn: string
+    const ttlSeconds: int64
+    const maxCacheSize: Types.PositiveInteger
     const grantTokens: KMS.GrantTokenList
+    const cryptoPrimitives: Primitives.AtomicPrimitivesClient
+    const branchKeyStoreIndex: string
 
     predicate ValidState()
       ensures ValidState() ==> History in Modifies
@@ -86,67 +110,100 @@ module AwsKmsHierarchicalKeyring {
       && History in Modifies
       && kmsClient.ValidState()
       && ddbClient.ValidState()
+      && cryptoPrimitives.ValidState()
       && kmsClient.Modifies <= Modifies
       && ddbClient.Modifies <= Modifies
+      && cryptoPrimitives.Modifies <= Modifies
       && History !in kmsClient.Modifies
       && History !in ddbClient.Modifies
+      && History !in cryptoPrimitives.Modifies
+      // TODO this should eventually be Valid branch key store arn
+      && DDB.IsValid_TableName(this.branchKeyStoreArn)
+      && DDB.IsValid_IndexName(this.branchKeyStoreIndex)
     }
 
     constructor (
-      // MUST provide and MUST NOT be null.
+      //= aws-encryption-sdk-specification/framework/aws-kms/aws-kms-hierarchical-keyring.md#initialization
+      //= type=implication
+      //# - MUST provide an AWS KMS SDK client
       kmsClient: KMS.IKeyManagementServiceClient,
-      // MUST provide
+      //= aws-encryption-sdk-specification/framework/aws-kms/aws-kms-hierarchical-keyring.md#initialization
+      //= type=implication
+      //# - MUST provide an AWS KMS key identifier
       awsKmsKey: string,
-      // MAY provide a list of grant tokens
+      //= aws-encryption-sdk-specification/framework/aws-kms/aws-kms-hierarchical-keyring.md#initialization
+      //= type=implication
+      //# - MAY provide a list of Grant Tokens
       grantTokens: KMS.GrantTokenList,
-
-      // MUST provide and MUST NOT be null
+      //= aws-encryption-sdk-specification/framework/aws-kms/aws-kms-hierarchical-keyring.md#initialization
+      //= type=implication
+      //# - MUST provide an AWS DDB SDK client
       ddbClient: DDB.IDynamoDB_20120810Client,
-      // MUST provide
-      branchKeysTableName: string,
-      // MUST provide
+      //= aws-encryption-sdk-specification/framework/aws-kms/aws-kms-hierarchical-keyring.md#initialization
+      //= type=implication
+      //# - MUST provide an AWS DDB Table ARN
+      branchKeyStoreArn: string,
+      //= aws-encryption-sdk-specification/framework/aws-kms/aws-kms-hierarchical-keyring.md#initialization
+      //= type=implication
+      //# - MUST provide a Branch Key Identifier
       branchKeyId: string,
-      // MAY provide
-      ttlMilliseconds: int64,
-
-      maxCacheSize: int32
+      //= aws-encryption-sdk-specification/framework/aws-kms/aws-kms-hierarchical-keyring.md#initialization
+      //= type=implication
+      //# - MUST provide a cache limit TTL
+      ttlSeconds: int64,
+      //= aws-encryption-sdk-specification/framework/aws-kms/aws-kms-hierarchical-keyring.md#initialization
+      //= type=implication
+      //# - MAY provide a max cache size
+      maxCacheSize: Types.PositiveInteger,
+      cryptoPrimitives : Primitives.AtomicPrimitivesClient
     )
+      //= aws-encryption-sdk-specification/framework/aws-kms/aws-kms-hierarchical-keyring.md#initialization
+      //= type=implication
+      //# The AWS KMS
+      //# key identifier MUST be [a valid identifier](aws-kms-key-arn.md#a-
+      //# valid-aws-kms-identifier).
       requires ParseAwsKmsIdentifier(awsKmsKey).Success?
       requires UTF8.IsASCIIString(awsKmsKey)
       requires 0 < |awsKmsKey| <= MAX_AWS_KMS_IDENTIFIER_LENGTH
-      requires DDB.IsValid_TableName(branchKeysTableName)
-      requires kmsClient.ValidState() && ddbClient.ValidState()
       requires maxCacheSize >= 1
+      requires DDB.IsValid_TableName(branchKeyStoreArn)
+      requires kmsClient.ValidState() && ddbClient.ValidState() && cryptoPrimitives.ValidState()
       ensures
-        && this.kmsClient           == kmsClient
-        && this.awsKmsKey           == awsKmsKey
-        && this.grantTokens         == grantTokens
-        && this.ddbClient           == ddbClient
-        && this.branchKeysTableName == branchKeysTableName
-        && this.branchKeyId         == branchKeyId
-        && this.ttlMilliseconds     == ttlMilliseconds
-        && this.maxCacheSize        == maxCacheSize
-      ensures ValidState() && fresh(this) && fresh(History) && fresh(Modifies - kmsClient.Modifies - ddbClient.Modifies)
+        && this.kmsClient    == kmsClient
+        && this.awsKmsKey    == awsKmsKey
+        && this.grantTokens  == grantTokens
+        && this.ddbClient    == ddbClient
+        && this.branchKeyStoreArn  == branchKeyStoreArn
+        && this.branchKeyId  == branchKeyId
+        && this.ttlSeconds   == ttlSeconds
+        && this.maxCacheSize == maxCacheSize
+      ensures ValidState() && fresh(this) && fresh(History) && fresh(Modifies - kmsClient.Modifies - ddbClient.Modifies - cryptoPrimitives.Modifies)
     {
       var parsedAwsKmsId    := ParseAwsKmsIdentifier(awsKmsKey);
-
+      // TODO add DDB Table Arn Parsing
       this.kmsClient           := kmsClient;
       this.awsKmsKey           := awsKmsKey;
       this.awsKmsArn           := parsedAwsKmsId.value;
       this.grantTokens         := grantTokens;
       this.ddbClient           := ddbClient;
-      this.branchKeysTableName := branchKeysTableName;
+      this.branchKeyStoreArn   := branchKeyStoreArn;
       this.branchKeyId         := branchKeyId;
-      this.ttlMilliseconds     := ttlMilliseconds;
+      this.ttlSeconds          := ttlSeconds;
       this.maxCacheSize        := maxCacheSize;
+      this.cryptoPrimitives    := cryptoPrimitives;
+      this.branchKeyStoreIndex := BRANCH_KEY_STORE_GSI;
       
       History := new Types.IKeyringCallHistory();
-      Modifies := {History} + kmsClient.Modifies + ddbClient.Modifies;
+      Modifies := {History} + kmsClient.Modifies + ddbClient.Modifies + cryptoPrimitives.Modifies;
     }
 
 
     predicate OnEncryptEnsuresPublicly ( input: Types.OnEncryptInput , output: Result<Types.OnEncryptOutput, Types.Error> ) {true}
     
+    //= aws-encryption-sdk-specification/framework/aws-kms/aws-kms-hierarchical-keyring.md#onencrypt
+    //= type=implication
+    //# OnEncrypt MUST take [encryption materials]
+    //# (../structures.md#encryption-materials) as input.
     method OnEncrypt'(input: Types.OnEncryptInput)
       returns (res: Result<Types.OnEncryptOutput, Types.Error>)
       requires ValidState()
@@ -161,15 +218,101 @@ module AwsKmsHierarchicalKeyring {
           input.materials,
           res.value.materials
         )
-      ensures StringifyEncryptionContext(input.materials.encryptionContext).Failure?
-      ==>
-        res.Failure?
 
       ensures !KMS.IsValid_KeyIdType(awsKmsKey)
       ==>
         res.Failure?
     {
-      return Failure(Types.AwsCryptographicMaterialProvidersException(message := "Add Hierarchical Crypto Operation Logic"));
+      var materials := input.materials;
+      var suite := materials.algorithmSuite;
+      var aad :- EncryptionContextToAADHierarchy(materials.encryptionContext);
+
+      var plaintextDataKey := materials.plaintextDataKey.UnwrapOr([]);
+
+      if plaintextDataKey == [] {
+        var randomKeyResult := cryptoPrimitives
+          .GenerateRandomBytes(Crypto.GenerateRandomBytesInput(length := GetEncryptKeyLength(suite)));
+        var k' :- randomKeyResult.MapFailure(e => Types.AwsCryptographyPrimitives(AwsCryptographyPrimitives := e));
+        plaintextDataKey := k';
+      }
+      
+      var branchKeyIdUtf8 :- UTF8.Encode(this.branchKeyId)
+        .MapFailure(WrapStringToError);
+      
+      //= aws-encryption-sdk-specification/framework/aws-kms/aws-kms-hierarchical-keyring.md#onencrypt
+      //= type=implication
+      //# The hierarchical keyring MUST attempt to obtain the hierarchical materials by querying 
+      //# the backing branch keystore
+      var hierarchicalMaterials :- GetActiveHierarchicalMaterials(branchKeyId, branchKeyIdUtf8);
+      
+      var branchKey := hierarchicalMaterials.branchKey;
+      // TODO: determine the uuid byte encoding instead of the utf8 encoding
+      var branchKeyVersion := hierarchicalMaterials.branchKeyVersion;
+      
+      //= aws-encryption-sdk-specification/framework/aws-kms/aws-kms-hierarchical-keyring.md#branch-key-wrapping
+      //# The hierarchical keyring MUST:
+      // (blank line for duvet)
+      //# 1. Generate a 16 byte random salt using a secure source of randomness
+      //# 1. Generate a 12 byte random iv using a secure source of randomness
+      var maybeNonceSalt := cryptoPrimitives.GenerateRandomBytes(
+        Crypto.GenerateRandomBytesInput(length := H_WRAP_NONCE_LEN + H_WRAP_SALT_LEN)
+      );
+      var saltAndNonce :- maybeNonceSalt.MapFailure(e => Types.AwsCryptographyPrimitives(AwsCryptographyPrimitives := e));
+      
+      var salt := saltAndNonce[0..H_WRAP_SALT_LEN];
+      var nonce := saltAndNonce[H_WRAP_SALT_LEN..];
+      
+      //= aws-encryption-sdk-specification/framework/aws-kms/aws-kms-hierarchical-keyring.md#branch-key-wrapping-and-unwrapping-aad
+      //# the keyring MUST include the following values as part of the AAD for the AES Encrypt/Decrypt calls.
+      // (blank line for duvet)
+      // To construct the AAD, the keyring MUST concatante the following values
+      // (blank line for duvet)
+      //# 1. "aws-kms-hierarchy" as UTF8 Bytes
+      //# 1. Value of `branch-key-id` as UTF8 Bytes
+      //# 1. [version](../structures.md#branch-key-version) as Bytes
+      //# 1. [encryption context](structures.md#encryption-context-1) from the input
+      //#   [encryption materials](../structures.md#encryption-materials) in the same format as the serialization of
+      //#   [message header AAD key value pairs](../../data-format/message-header.md#key-value-pairs).
+      var wrappingAad := WrappingAad(branchKeyIdUtf8, branchKeyVersion, aad);
+      
+      var wrappedPdk :- BranchKeyWrapping(hierarchicalMaterials, plaintextDataKey, nonce, salt, wrappingAad, cryptoPrimitives);
+
+      // TODO above we wrapped a key according to the standard ESDK Hierarchy Spec
+      // For DBE we have to perform additional wrapping - coming in a followup PR
+      // TODO decode branchKeyVersion to get the plain bytes here instead of the UTF8 Bytes
+      var serializedEdk := salt + nonce + branchKeyVersion + wrappedPdk.cipherText + wrappedPdk.authTag;
+
+      var edk := Types.EncryptedDataKey(
+        //= aws-encryption-sdk-specification/framework/aws-kms/aws-kms-hierarchical-keyring.md#onencrypt
+        //= type=implication
+        //# [key provider id](../structures.md#key-provider-id): MUST be UTF8 Encoded "aws-kms-hierarchy"
+        keyProviderId := PROVIDER_ID_HIERARCHY,
+        //= aws-encryption-sdk-specification/framework/aws-kms/aws-kms-hierarchical-keyring.md#onencrypt
+        //= type=implication
+        //# [key provider info](../structures.md#key-provider-information): MUST be the UTF8 Encoded AWS DDB response `branch-key-id`
+        keyProviderInfo := branchKeyIdUtf8,
+        //= aws-encryption-sdk-specification/framework/aws-kms/aws-kms-hierarchical-keyring.md#onencrypt
+        //= type=implication
+        //# [ciphertext](../structures.md#ciphertext): MUST be serialized as the [hierarchical keyring ciphertext](#ciphertext)
+        ciphertext := serializedEdk
+      );
+
+      //= aws-encryption-sdk-specification/framework/aws-kms/aws-kms-hierarchical-keyring.md#onencrypt
+      //= type=implication
+      //# OnEncrypt MUST append a new [encrypted data key](../structures.md#encrypted-data-key)
+      //# to the encrypted data key list in the [encryption materials](../structures.md#encryption-materials)
+      :- Need(
+        // TODO add support
+        materials.algorithmSuite.symmetricSignature.None?,
+        E("Symmetric Signatures not yet implemented.")
+      );
+
+      var nextMaterials :- if materials.plaintextDataKey.None? then
+        Materials.EncryptionMaterialAddDataKey(materials, plaintextDataKey, [edk], None)
+      else
+        Materials.EncryptionMaterialAddEncryptedDataKeys(materials, [edk], None);
+      var result := Types.OnEncryptOutput(materials := nextMaterials);
+      return Success(result);
     }
 
     predicate OnDecryptEnsuresPublicly ( input: Types.OnDecryptInput , output: Result<Types.OnDecryptOutput, Types.Error> ) {true}
@@ -188,7 +331,675 @@ module AwsKmsHierarchicalKeyring {
           input.materials,
           res.value.materials)
     {
-      return Failure(Types.AwsCryptographicMaterialProvidersException(message := "Add Hierarchical Crypto Operation Logic"));
+      var materials := input.materials;
+      var suite := input.materials.algorithmSuite;
+
+      :- Need(
+        Materials.DecryptionMaterialsWithoutPlaintextDataKey(materials),
+        E("Keyring received decryption materials that already contain a plaintext data key.")
+      );
+      
+      var filter := new OnDecryptHierarchyEncryptedDataKeyFilter(branchKeyId);
+      var edksToAttempt :- FilterWithResult(filter, input.encryptedDataKeys);
+
+      :- Need(
+        0 < |edksToAttempt|,
+        E("Unable to decrypt data key: No Encrypted Data Keys found to match.")
+      );
+    
+      var aad :- EncryptionContextToAADHierarchy(materials.encryptionContext);
+      var decryptClosure := new DecryptSingleEncryptedDataKey(
+        materials,
+        aad,
+        kmsClient,
+        ddbClient,
+        cryptoPrimitives,
+        branchKeyStoreArn,
+        branchKeyId,
+        awsKmsKey,
+        grantTokens
+      );
+
+      var outcome, attempts := ReduceToSuccess(
+        decryptClosure,
+        edksToAttempt
+      );
+
+      var SealedDecryptionMaterials :- outcome
+        //= aws-encryption-sdk-specification/framework/aws-kms/aws-kms-keyring.md#ondecrypt
+        //# If OnDecrypt fails to successfully decrypt any [encrypted data key]
+        //# (../structures.md#encrypted-data-key), then it MUST yield an error
+        //# that includes all the collected errors.
+        .MapFailure(errors => Types.Collection( list := errors));
+      
+      assert decryptClosure.Ensures(Last(attempts).input, Success(SealedDecryptionMaterials), DropLast(attempts));
+      return Success(Types.OnDecryptOutput(
+        materials := SealedDecryptionMaterials
+      ));
+    }
+
+    method GetActiveHierarchicalMaterials(
+      branchKeyId: string,
+      branchKeyIdUtf8: seq<uint8>
+    )
+      returns (material: Result<Types.HierarchicalMaterials, Types.Error>)
+      requires ValidState()
+      modifies ddbClient.Modifies, kmsClient.Modifies, cryptoPrimitives.Modifies
+      ensures ValidState()
+    {
+      var expressionAttributeValues : DDB.AttributeMap := map[
+        EXPRESSION_ATTRIBUTE_VALUE_STATUS_KEY := DDB.AttributeValue.S(EXPRESSION_ATTRIBUTE_VALUE_STATUS_VALUE),
+        EXPRESSION_ATTRIBUTE_VALUE_BRANCH_KEY := DDB.AttributeValue.S(branchKeyId)
+      ];
+
+      //= aws-encryption-sdk-specification/framework/aws-kms/aws-kms-hierarchical-keyring.md#query-branch-keystore-onencrypt
+      //= type=implication
+      //# To query this keystore, the caller MUST do the following:
+      var queryInput := DDB.QueryInput(
+        TableName := branchKeyStoreArn,
+        //= aws-encryption-sdk-specification/framework/aws-kms/aws-kms-hierarchical-keyring.md#query-branch-keystore-onencrypt
+        //= type=implication
+        //# To query this keystore, the caller MUST do the following:
+        // (blank line for duvet)
+        //# Use the global secondary index (GSI) Active-Keys to query the keystore to retrieve the active key 
+        //# that matches the branch-key-id configured on the keyring. 
+        IndexName := Some(BRANCH_KEY_STORE_GSI),
+        Select := None(),
+        AttributesToGet := None(),
+        Limit := None(),
+        ConsistentRead :=  None() ,
+        KeyConditions := None(),
+        QueryFilter := None(),
+        ConditionalOperator := None(),
+        ScanIndexForward := None(),
+        ExclusiveStartKey := None(),
+        ReturnConsumedCapacity :=  None(),
+        ProjectionExpression := None(),
+        FilterExpression := None(),
+        KeyConditionExpression := Some(KEY_CONDITION_EXPRESSION),
+        ExpressionAttributeNames := Some(EXPRESSION_ATTRIBUTE_NAMES),
+        ExpressionAttributeValues := Some(expressionAttributeValues)
+      );
+
+      var maybeQueryResponse := ddbClient.Query(queryInput);
+      var queryResponse :- maybeQueryResponse
+        .MapFailure(e => Types.ComAmazonawsDynamodb(ComAmazonawsDynamodb := e));
+      
+      :- Need(
+        && queryResponse.Items.Some?
+        && |queryResponse.Items.value| > 0,
+        E("No item found for corresponding branch key identifier.")
+      );
+
+      //= aws-encryption-sdk-specification/framework/aws-kms/aws-kms-hierarchical-keyring.md#query-branch-keystore-onencrypt
+      //= type=implication
+      //# The AWS DDB response MUST contain the fields defined in the [branch keystore record format](../branch-key-store.md#record-format).
+      //# If the record does not contain the defined fields, OnEncrypt MUST fail.
+      :- Need(
+        branchKeyItemHasRequiredAttributes?(queryResponse.Items.value[0]),
+        E("Malformed Branch Key entry")
+      );
+
+      // TODO resolve the one to take by using the create-time value
+      // if we have an active-active case we should resolve the version to use 
+      // by looking at the `create-time` value
+      var branchKeyRecord: branchKeyItem := queryResponse.Items.value[0];
+
+      //= aws-encryption-sdk-specification/framework/aws-kms/aws-kms-hierarchical-keyring.md#aws-kms-branch-key-decryption
+      //= type=implication
+      //# The keyring MUST use the configured `KMS SDK Client` to decrypt the value of the branch key field.
+      var branchKeyResponse :- decryptBranchKey(branchKeyRecord, awsKmsKey, grantTokens, kmsClient);
+
+      // TODO figure out how to validate a uuid
+      // We should be able to convert this uuid string to the 16 byte representation      
+      var branchKeyUuidString: string := branchKeyRecord["version"].S;
+      var branchKeyUuidUtf8 :- UTF8.Encode(branchKeyUuidString)
+        .MapFailure(WrapStringToError);
+      
+      var branchKey : seq<uint8> := branchKeyResponse.Plaintext.value;
+      
+      var hierarchicalMaterials := Types.HierarchicalMaterials(
+        branchKey := branchKey,
+        branchKeyVersion := branchKeyUuidUtf8
+      );
+      
+      return Success(hierarchicalMaterials);
     }
   }
+
+  method decryptBranchKey(
+    branchKeyRecord: branchKeyItem,
+    awsKmsKey: AwsKmsIdentifierString,
+    grantTokens: KMS.GrantTokenList,
+    kmsClient: KMS.IKeyManagementServiceClient
+  )
+    returns (output: Result<KMS.DecryptResponse, Types.Error>)
+
+    requires branchKeyItemHasRequiredAttributes?(branchKeyRecord)
+    requires kmsClient.ValidState()
+    modifies kmsClient.Modifies
+    ensures kmsClient.ValidState()
+    ensures output.Success?
+      ==> 
+        && output.value.KeyId.Some?
+        && output.value.KeyId.value == awsKmsKey
+        && output.value.Plaintext.Some?
+        && 32 == |output.value.Plaintext.value|
+  {
+    //= aws-encryption-sdk-specification/framework/aws-kms/aws-kms-hierarchical-keyring.md#aws-kms-branch-key-decryption
+    //= type=implication
+    //# The keyring MUST create a branch key [encryption context](../structures.md#encryption-context) map using
+    //# each attribute name from the AWS DDB response except the `enc` attribute as a key and each corresponding
+    //# attribute value as the value of the KMS Encryption Context.
+    var wrappedBranchKey: KMS.CiphertextType := branchKeyRecord[BRANCH_KEY_FIELD].B;
+
+    var encCtxDdbMap := branchKeyRecord - {BRANCH_KEY_FIELD};
+
+    var encCtxMap: map<string, string> :=
+      map k <- encCtxDdbMap ::
+        k := ValueToString(encCtxDdbMap[k]).value; 
+    
+    var decryptRequest :=
+      //= aws-encryption-sdk-specification/framework/aws-kms/aws-kms-hierarchical-keyring.md#aws-kms-branch-key-decryption
+      //= type=implication
+      //# the keyring MUST call with a request constructed as follows: 
+      KMS.DecryptRequest(
+        //= aws-encryption-sdk-specification/framework/aws-kms/aws-kms-hierarchical-keyring.md#aws-kms-branch-key-decryption
+        //# - `KeyId` MUST be the configured AWS KMS key identifier.
+        KeyId := Some(awsKmsKey),
+        //= aws-encryption-sdk-specification/framework/aws-kms/aws-kms-hierarchical-keyring.md#aws-kms-branch-key-decryption
+        //# - `CiphertextBlob` MUST be the `enc` AWS DDB response value.
+        CiphertextBlob := wrappedBranchKey,
+        //= aws-encryption-sdk-specification/framework/aws-kms/aws-kms-hierarchical-keyring.md#aws-kms-branch-key-decryption
+        //# - `EncryptionContext` MUST be the branch key encryption context map.
+        EncryptionContext := Some(encCtxMap),
+        //= aws-encryption-sdk-specification/framework/aws-kms/aws-kms-hierarchical-keyring.md#aws-kms-branch-key-decryption
+        //# - `GrantTokens` MUST be this keyring's
+        //# [grant tokens](https://docs.aws.amazon.com/kms/latest/developerguide/concepts.html#grant_token).
+        GrantTokens := Some(grantTokens),
+        EncryptionAlgorithm := None
+      );
+
+    var maybeDecryptResponse := kmsClient.Decrypt(decryptRequest);
+    var decryptResponse :- maybeDecryptResponse
+      .MapFailure(e => Types.ComAmazonawsKms(ComAmazonawsKms := e));
+
+    :- Need(
+      && decryptResponse.KeyId.Some?
+      && decryptResponse.KeyId.value == awsKmsKey
+      && decryptResponse.Plaintext.Some?
+      && 32 == |decryptResponse.Plaintext.value|,
+      E("Invalid response from KMS Decrypt")
+    );
+    return Success(decryptResponse);
+  }
+
+  function method ValueToString(a: DDB.AttributeValue): Result<string, Types.Error>
+  {
+    // TODO: come back and agree on how we would like to represent 
+    // the other types. Look at DynamoToStruct.dfy to see how 
+    // DBE is doing this conversion.
+    // This is allowing us to bind the type of the value to the encryption context
+    // we pass to KMS; we could also do a runtime check to check for this
+    match a {
+      case S(s) => Success(a.S)
+      case N(n) => Success(a.N)
+      // For now we only support AttributeValues that are either String or Number
+      // AttributeValues, we have not specified how to represent attributes other than these
+      // two, we SHOULD include them but we have to agree how to turn the underlying
+      // type into a string/bytes so that they could be turned to UTF8 bytes to pass KMS.
+      case _ => Failure(Types.AwsCryptographicMaterialProvidersException(message := "Type not supported"))
+    }
+  }
+
+  method DeriveEncryptionKeyFromBranchKey(
+    branchKey: seq<uint8>,
+    salt: seq<uint8>,
+    purpose: Option<seq<uint8>>,
+    cryptoPrimitives: Primitives.AtomicPrimitivesClient
+  )
+    returns (output: Result<seq<uint8>, Types.Error>)
+
+    requires cryptoPrimitives.ValidState()
+    modifies cryptoPrimitives.Modifies
+    ensures cryptoPrimitives.ValidState()
+    ensures output.Success? ==> |output.value| == 32
+  {
+    //= aws-encryption-sdk-specification/framework/aws-kms/aws-kms-hierarchical-keyring.md#branch-key-wrapping
+    //# 3. Use a [KDF in Counter Mode with a Pseudo Random Function with HMAC SHA 256]
+    //# (https://nvlpubs.nist.gov/nistpubs/SpecialPublications/NIST.SP.800-108r1.pdf) 
+    var maybeDerivedBranchKey := cryptoPrimitives.KdfCounterMode(
+      Crypto.KdfCtrInput(
+        digestAlgorithm := Crypto.DigestAlgorithm.SHA_256,
+        //= aws-encryption-sdk-specification/framework/aws-kms/aws-kms-hierarchical-keyring.md#branch-key-wrapping
+        //# - Use the branch key as the `key`.
+        ikm := branchKey,
+        //= aws-encryption-sdk-specification/framework/aws-kms/aws-kms-hierarchical-keyring.md#branch-key-wrapping
+        //# to derive a 32 byte `derivedBranchKey`
+        expectedLength := DERIVED_BRANCH_KEY_EXPECTED_LENGTH,
+        // TODO: change name to label
+        purpose := purpose,
+        //= aws-encryption-sdk-specification/framework/aws-kms/aws-kms-hierarchical-keyring.md#branch-key-wrapping
+        //# - Use the `salt` as the salt.
+        nonce := Some(salt)
+      )
+    );
+    var derivedBranchKey :- maybeDerivedBranchKey.MapFailure(e => Types.AwsCryptographyPrimitives(AwsCryptographyPrimitives := e));
+    output := Success(derivedBranchKey);
+  }
+
+  method BranchKeyWrapping(
+    hierarchicalMaterials: Types.HierarchicalMaterials,
+    pdk: seq<uint8>,
+    iv: seq<uint8>,
+    salt: seq<uint8>,
+    aad: seq<uint8>,
+    cryptoPrimitives: Primitives.AtomicPrimitivesClient
+  )
+    returns (output: Result<Crypto.AESEncryptOutput, Types.Error>)
+    requires cryptoPrimitives.ValidState()
+    modifies cryptoPrimitives.Modifies
+    ensures cryptoPrimitives.ValidState()
+  {
+    var derivedBranchKey :- DeriveEncryptionKeyFromBranchKey(
+      hierarchicalMaterials.branchKey,
+      salt,
+      Some(PROVIDER_ID_HIERARCHY),
+      cryptoPrimitives
+    );
+    var maybeWrappedPdk := cryptoPrimitives.AESEncrypt(
+      Crypto.AESEncryptInput(
+        //= aws-encryption-sdk-specification/framework/aws-kms/aws-kms-hierarchical-keyring.md#branch-key-wrapping
+        //= type=implication
+        //# 1. Encrypt a plaintext data key with the `derivedBranchKey` using
+        //# `AES-GCM-256` with the following inputs:
+        encAlg := AES_256_ENC_ALG,
+        //= aws-encryption-sdk-specification/framework/aws-kms/aws-kms-hierarchical-keyring.md#branch-key-wrapping
+        //= type=implication
+        //# MUST use the derived `IV` as the AES-GCM IV.  
+        iv := iv,
+        //= aws-encryption-sdk-specification/framework/aws-kms/aws-kms-hierarchical-keyring.md#branch-key-wrapping
+        //= type=implication
+        //# MUST use the `derivedBranchKey` as the AES-GCM cipher key.
+        key := derivedBranchKey,
+        //= aws-encryption-sdk-specification/framework/aws-kms/aws-kms-hierarchical-keyring.md#branch-key-wrapping
+        //= type=implication
+        //# MUST use the plain text data key that will be wrapped by the `derivedBranchKey` as the AES-GCM message.
+        msg := pdk ,
+        //= aws-encryption-sdk-specification/framework/aws-kms/aws-kms-hierarchical-keyring.md#branch-key-wrapping
+        //= type=implication
+        //# - MUST use the serialized [AAD](#branch-key-wrapping-and-unwrapping-aad) as the AES-GCM AAD.
+        aad := aad
+      )
+    );
+    var wrappedPdk :- maybeWrappedPdk.MapFailure(e => Types.AwsCryptographyPrimitives(AwsCryptographyPrimitives := e));
+    output := Success(wrappedPdk);
+  }
+
+  method BranchKeyUnwrapping(
+    hierarchicalMaterials: Types.HierarchicalMaterials,
+    ciphertext: seq<uint8>,
+    iv: seq<uint8>,
+    salt: seq<uint8>,
+    aad: seq<uint8>,
+    authTag: seq<uint8>,
+    cryptoPrimitives: Primitives.AtomicPrimitivesClient
+  )
+    returns (output: Result<seq<uint8>, Types.Error>)
+    requires cryptoPrimitives.ValidState()
+    modifies cryptoPrimitives.Modifies
+    ensures cryptoPrimitives.ValidState()
+  {
+    var derivedBranchKey :- DeriveEncryptionKeyFromBranchKey(
+      hierarchicalMaterials.branchKey,
+      salt,
+      Some(PROVIDER_ID_HIERARCHY),
+      cryptoPrimitives);
+    var maybeUnwrappedPdk :=  cryptoPrimitives.AESDecrypt(
+      Crypto.AESDecryptInput(
+        encAlg := AES_256_ENC_ALG,
+        key := derivedBranchKey,
+        cipherTxt := ciphertext,
+        authTag := authTag, 
+        iv := iv,
+        aad := aad
+      )
+    );
+    var unwrappedPdk :- maybeUnwrappedPdk.MapFailure(e => Types.AwsCryptographyPrimitives(AwsCryptographyPrimitives := e));
+    output := Success(unwrappedPdk);
+  }
+
+  //=  aws-encryption-sdk-specification/framework/raw-aes-keyring.md#onencrypt
+  //# The keyring MUST attempt to serialize the [encryption materials']
+  //# (structures.md#encryption-materials) [encryption context]
+  //# (structures.md#encryption-context-1) in the same format as the
+  //# serialization of [message header AAD key value pairs](../data-format/
+  //# message-header.md#key-value-pairs).
+  // TODO: Tests/proofs
+  // TODO move to CanonicalEncryptionContext.dfy
+  function method EncryptionContextToAADHierarchy(
+    encryptionContext: Types.EncryptionContext
+  ):
+    (res: Result<seq<uint8>, Types.Error>)
+  {
+    :- Need(
+      |encryptionContext| < UINT16_LIMIT,
+      E("Encryption Context is too large")
+    );
+    var keys := SetToOrderedSequence(encryptionContext.Keys, UInt.UInt8Less);
+
+    if |keys| == 0 then
+      // TODO: this adheres to spec (message-header.md) but diverges from what we do
+      // in EncryptionContext.WriteAADSection
+      Success([])
+    else
+      var KeyIntoPairBytes := k
+        requires k in encryptionContext
+      =>
+        var v := encryptionContext[k];
+        :- Need(
+          HasUint16Len(k) && HasUint16Len(v),
+          E("Unable to serialize encryption context")
+        );
+        Success(UInt16ToSeq(|k| as uint16) + k + UInt16ToSeq(|v| as uint16) + v);
+
+      var pairsBytes :- Seq.MapWithResult(KeyIntoPairBytes, keys);
+
+      // The final return should be the bytes of the pairs, prepended with the number of pairs
+      var allBytes := UInt16ToSeq(|keys| as uint16) + Seq.Flatten(pairsBytes);
+      Success(allBytes)
+  }
+
+  method WrappingAad(
+    branchKeyId: seq<uint8>,
+    branchKeyVersion: seq<uint8>,
+    aad: seq<uint8>
+  )
+    returns (res : seq<uint8>)
+    requires UTF8.ValidUTF8Seq(branchKeyId)
+    // TODO right now branchKeyVersion is stored as UTF8 Bytes in the materials
+    // I either have to 1) decode the version every single time to get the raw uuid
+    // or 2). store it as raw bytes in the materials so that I can encode it once per call.
+  {
+      //= aws-encryption-sdk-specification/framework/aws-kms/aws-kms-hierarchical-keyring.md#branch-key-wrapping-and-unwrapping-aad
+      //= type=implication
+      //# To construct the AAD, the keyring MUST concatante the following values
+      // (blank line for duvet)
+      //# 1. "aws-kms-hierarchy" as UTF8 Bytes
+      //# 1. Value of `branch-key-id` as UTF8 Bytes
+      //# 1. [version](../structures.md#branch-key-version) as Bytes
+      //# 1. [encryption context](structures.md#encryption-context-1) from the input
+      //# [encryption materials](../structures.md#encryption-materials) in the same format as the serialization of
+      //# [message header AAD key value pairs](../../data-format/message-header.md#key-value-pairs).
+      var wraapingAad := PROVIDER_ID_HIERARCHY + branchKeyId + branchKeyVersion + aad;
+      return wraapingAad;
+  }
+  
+  class OnDecryptHierarchyEncryptedDataKeyFilter
+    extends DeterministicActionWithResult<Types.EncryptedDataKey, bool, Types.Error>
+  {
+    const branchKeyId: string
+
+    constructor(
+      branchKeyId: string
+    )
+    {
+      this.branchKeyId := branchKeyId;
+    }
+
+    predicate Ensures(
+      edk: Types.EncryptedDataKey,
+      res: Result<bool, Types.Error>
+    ) {
+      && (
+          && res.Success?
+          && res.value
+        ==>
+          edk.keyProviderId == PROVIDER_ID_HIERARCHY)
+    }
+
+    method Invoke(edk: Types.EncryptedDataKey)
+      returns (res: Result<bool, Types.Error>)
+      ensures Ensures(edk, res)
+    {
+      var providerInfo := edk.keyProviderInfo;
+      var providerId := edk.keyProviderId;
+
+      //= aws-encryption-sdk-specification/framework/aws-kms/aws-kms-hierarchical-keyring.md#ondecrypt
+      //= type=implication
+      //# - Its provider ID MUST match the UTF8 Encoded value of “aws-kms-hierarchy”.
+      if providerId != PROVIDER_ID_HIERARCHY {
+        return Success(false);
+      }
+      
+      if !UTF8.ValidUTF8Seq(providerInfo) {
+        // The Keyring produces UTF8 keyProviderInfo.
+        // If an `aws-kms-hierarchy` encrypted data key's keyProviderInfo is not UTF8
+        // this is an error, not simply an EDK to filter out.
+        return Failure(E("Invalid encoding, provider info is not UTF8."));
+      }
+
+      //= aws-encryption-sdk-specification/framework/aws-kms/aws-kms-hierarchical-keyring.md#ondecrypt
+      //# -- The deserialized key provider info MUST be UTF8 Decoded
+      var branchKeyId :- UTF8.Decode(providerInfo).MapFailure(WrapStringToError);
+      
+      //= aws-encryption-sdk-specification/framework/aws-kms/aws-kms-hierarchical-keyring.md#ondecrypt
+      //#  MUST match this keyring's configured `Branch Key Identifier`.
+      return Success(this.branchKeyId == branchKeyId);
+    }
+  }
+
+  class DecryptSingleEncryptedDataKey
+    extends ActionWithResult<
+      Types.EncryptedDataKey,
+      Materials.SealedDecryptionMaterials,
+      Types.Error>
+  {
+    const materials: Materials.DecryptionMaterialsPendingPlaintextDataKey
+    const aad: seq<uint8>
+    const kmsClient: KMS.IKeyManagementServiceClient
+    const ddbClient: DDB.IDynamoDB_20120810Client
+    const cryptoPrimitives: Primitives.AtomicPrimitivesClient
+    const branchKeyStoreArn: string
+    const branchKeyId: string
+    const awsKmsKey: AwsKmsIdentifierString
+    const grantTokens: KMS.GrantTokenList
+
+    constructor(
+      materials: Materials.DecryptionMaterialsPendingPlaintextDataKey,
+      aad: seq<uint8>,
+      kmsClient: KMS.IKeyManagementServiceClient,
+      ddbClient: DDB.IDynamoDB_20120810Client,
+      cryptoPrimitives: Primitives.AtomicPrimitivesClient,
+      branchKeyStoreArn: string,
+      branchKeyId: string,
+      awsKmsKey: AwsKmsIdentifierString,
+      grantTokens: KMS.GrantTokenList
+    )
+      requires ParseAwsKmsIdentifier(awsKmsKey).Success?
+      requires UTF8.IsASCIIString(awsKmsKey)
+      requires 0 < |awsKmsKey| <= MAX_AWS_KMS_IDENTIFIER_LENGTH
+      requires DDB.IsValid_TableName(branchKeyStoreArn)
+      requires kmsClient.ValidState() && ddbClient.ValidState() && cryptoPrimitives.ValidState()
+      ensures
+      && this.materials == materials
+      && this.aad       == aad
+      && this.kmsClient == kmsClient
+      && this.ddbClient == ddbClient
+      && this.cryptoPrimitives == cryptoPrimitives
+      && this.branchKeyStoreArn     == branchKeyStoreArn
+      && this.branchKeyId == branchKeyId
+      && this.awsKmsKey == awsKmsKey
+      && this.grantTokens == grantTokens
+      ensures Invariant()
+    {
+      this.materials := materials;
+      this.aad       := aad;
+      this.kmsClient := kmsClient;
+      this.ddbClient := ddbClient;
+      this.cryptoPrimitives := cryptoPrimitives;
+      this.branchKeyStoreArn := branchKeyStoreArn;
+      this.branchKeyId := branchKeyId;
+      this.awsKmsKey := awsKmsKey;
+      this.grantTokens := grantTokens;
+      Modifies := kmsClient.Modifies + ddbClient.Modifies + cryptoPrimitives.Modifies;
+    }
+
+    predicate Invariant()
+      reads Modifies
+      decreases Modifies
+    {
+      && kmsClient.ValidState()
+      && ddbClient.ValidState()
+      && cryptoPrimitives.ValidState()
+      && DDB.IsValid_TableName(this.branchKeyStoreArn)
+      && kmsClient.Modifies + ddbClient.Modifies + cryptoPrimitives.Modifies == Modifies
+    }
+
+    predicate Ensures(
+      edk: Types.EncryptedDataKey,
+      res: Result<Materials.SealedDecryptionMaterials, Types.Error>,
+      attemptsState: seq<ActionInvoke<Types.EncryptedDataKey, Result<Materials.SealedDecryptionMaterials, Types.Error>>>
+    )
+      reads Modifies
+      decreases Modifies
+    {
+      // TODO look at the KMS keyring to see how we ensure that the call
+      // to KMS was done correctly; this might be hard to prove once we add the cache
+      // but we should be able to do it.
+        res.Success?
+      ==>
+        && Invariant()
+        && KMS.IsValid_CiphertextType(edk.ciphertext)
+        && Materials.DecryptionMaterialsTransitionIsValid(materials, res.value)
+
+    }
+    method Invoke(
+      edk: Types.EncryptedDataKey,
+      // aad: seq<uint8>,
+      ghost attemptsState: seq<ActionInvoke<Types.EncryptedDataKey, Result<Materials.SealedDecryptionMaterials, Types.Error>>>
+    ) returns (res: Result<Materials.SealedDecryptionMaterials, Types.Error>)
+      requires Invariant()
+      modifies Modifies
+      decreases Modifies
+      ensures Invariant()
+      ensures Ensures(edk, res, attemptsState)
+    {
+      :- Need (
+        // Salt = 16, IV = 12, Version = 36, Encrypted Key = 32, Authentication Tag = 16
+        && |edk.ciphertext| == EXPECTED_EDK_CIPHERTEXT_LENGTH
+        && UTF8.ValidUTF8Seq(edk.keyProviderInfo),
+        Types.AwsCryptographicMaterialProvidersException(message := "Received EDK Ciphertext of incorrect length.")
+      );
+
+      var suite := materials.algorithmSuite;
+
+      var keyProviderId := edk.keyProviderId;
+      var branchKeyIdUtf8 := edk.keyProviderInfo;
+      var ciphertext := edk.ciphertext;
+
+      var salt := ciphertext[0..H_WRAP_SALT_LEN];
+      var iv := ciphertext[H_WRAP_SALT_LEN..EDK_CIPHERTEXT_BRANCH_KEY_VERSION_INDEX];
+      var branchKeyVersionUuid := ciphertext[EDK_CIPHERTEXT_BRANCH_KEY_VERSION_INDEX..EDK_CIPHERTEXT_VERSION_INDEX];
+      var wrappedKey := ciphertext[EDK_CIPHERTEXT_VERSION_INDEX..EDK_CIPHERTEXT_KEY_INDEX];
+      var authTag := ciphertext[EDK_CIPHERTEXT_KEY_INDEX..];
+      
+      var hierarchicalMaterials :- GetHierarchicalMaterialsVersion(branchKeyId, branchKeyIdUtf8, branchKeyVersionUuid);
+      var branchKey := hierarchicalMaterials.branchKey;
+      var branchKeyVersionUtf8 := hierarchicalMaterials.branchKeyVersion;
+      
+      var wrappingAad := WrappingAad(branchKeyIdUtf8, branchKeyVersionUtf8, aad);
+      var pdk :- BranchKeyUnwrapping(hierarchicalMaterials, wrappedKey, iv, salt, wrappingAad, authTag, cryptoPrimitives);
+
+      :- Need(
+        |pdk| == AES_256_ENC_KEY_LENGTH as int, 
+        E("Unable to decrypt wrapped data key.")
+      );
+      
+      // TODO add support
+      :- Need(
+        materials.algorithmSuite.symmetricSignature.None?,
+        E("Symmetric Signatures not yet implemented.")
+      );
+
+      var result :- Materials.DecryptionMaterialsAddDataKey(materials, pdk, None);
+      return Success(result);
+    }
+
+    method GetHierarchicalMaterialsVersion(
+      branchKeyId: string,
+      branchKeyIdUtf8: seq<uint8>,
+      branchKeyVersion: seq<uint8>
+    )
+      returns (material: Result<Types.HierarchicalMaterials, Types.Error>)
+      // TODO Define valid HierarchicalMaterials such that we can ensure they are correct
+      requires Invariant()
+      requires ddbClient.ValidState() && kmsClient.ValidState() && cryptoPrimitives.ValidState()
+      modifies ddbClient.Modifies, kmsClient.Modifies, cryptoPrimitives.Modifies
+      ensures ddbClient.ValidState() && kmsClient.ValidState() && cryptoPrimitives.ValidState()
+    {
+      var version :- UTF8.Decode(branchKeyVersion).MapFailure(WrapStringToError);
+
+      var dynamoDbKey: DDB.Key := map[
+        BRANCH_KEY_IDENTIFIER_FIELD := DDB.AttributeValue.S(branchKeyId),
+        VERSION_FIELD := DDB.AttributeValue.S(version)
+      ];
+
+      var ItemRequest := DDB.GetItemInput(
+        Key := dynamoDbKey,
+        TableName := branchKeyStoreArn,
+        AttributesToGet := None(),
+        ConsistentRead :=  None(),
+        ReturnConsumedCapacity := None(),
+        ProjectionExpression := None(),
+        ExpressionAttributeNames := None() 
+      );
+
+      var maybeGetItem := ddbClient.GetItem(ItemRequest);
+      var getItemResponse :- maybeGetItem
+        .MapFailure(e => Types.ComAmazonawsDynamodb(ComAmazonawsDynamodb := e));
+      
+      :- Need(
+        getItemResponse.Item.Some?,
+        E("No item found for corresponding branch key identifier.")
+      );
+
+      //= aws-encryption-sdk-specification/framework/aws-kms/aws-kms-hierarchical-keyring.md#query-branch-keystore-onencrypt
+      //= type=implication
+      //# The AWS DDB response MUST contain the fields defined in the [branch keystore record format](../branch-key-store.md#record-format).
+      //# If the record does not contain the defined fields, OnEncrypt MUST fail.
+      :- Need(
+        branchKeyItemHasRequiredAttributes?(getItemResponse.Item.value),
+        E("Malformed Branch Key entry")
+      );
+ 
+      var branchKeyRecord: branchKeyItem := getItemResponse.Item.value;
+
+      var maybeBranchKeyResponse := decryptBranchKey(branchKeyRecord, awsKmsKey, grantTokens, kmsClient);
+      var branchKeyResponse :- maybeBranchKeyResponse;
+
+      var branchKeyUuidString: string := branchKeyRecord[VERSION_FIELD].S;
+      var branchKeyUuid :- UTF8.Encode(branchKeyUuidString)
+        .MapFailure(WrapStringToError);
+      
+      var branchKey : seq<uint8> := branchKeyResponse.Plaintext.value;
+      
+      var hierarchicalMaterials := Types.HierarchicalMaterials(
+        branchKey := branchKey, 
+        branchKeyVersion := branchKeyUuid
+      );
+      
+      return Success(hierarchicalMaterials);
+    }
+
+  }
+
+  function method SerializeEDKCiphertext(encOutput: Crypto.AESEncryptOutput): (ciphertext: seq<uint8>) {
+    encOutput.cipherText + encOutput.authTag
+  }
+
+  function method E(s : string) : Types.Error {
+    Types.AwsCryptographicMaterialProvidersException(message := s)
+  }
+
 }
