AwsCryptographicMaterialProviders/test/Keyrings/AwsKms/AwsKmsHierarchicalKeyring/TestAwsKmsHierarchicalKeyring.dfy
@@ -1,0 +1,86 @@
+// Copyright Amazon.com Inc. or its affiliates. All Rights Reserved.
+// SPDX-License-Identifier: Apache-2.0
+
+include "../../../../src/Index.dfy"
+include "../../../TestUtils.dfy"
+
+
+module TestAwsKmsHierarchicalKeyring {
+  import Types = AwsCryptographyMaterialProvidersTypes
+  import ComAmazonawsKmsTypes
+  import KMS = Com.Amazonaws.Kms
+  import DDB = Com.Amazonaws.Dynamodb
+  import MaterialProviders
+  import opened TestUtils
+  import opened UInt = StandardLibrary.UInt
+  import opened Wrappers
+
+  method {:test} TestClientWithHierarchy()
+  {
+    var mpl :- expect MaterialProviders.MaterialProviders();
+    var kmsClient :- expect KMS.KMSClient();
+    var dynamodbClient :- expect DDB.DynamoDBClient();
+    var ttl : int64 := (1 * 60000) * 10;
+    // THIS IS A TESTING RESOURCE DO NOT USE IN A PRODUCTION ENVIRONMENT
+    var keyArn := "arn:aws:kms:us-west-2:370957321024:key/9d989aa2-2f9c-438c-a745-cc57d3ad0126";
+
+    var hierarchyKeyringResult := mpl.CreateAwsKmsHierarchicalKeyring(
+      Types.CreateAwsKmsHierarchicalKeyringInput(
+        branchKeyId := "hierarchy-test-v1",
+        kmsKeyId := keyArn,
+        kmsClient := kmsClient,
+        ddbClient := dynamodbClient,
+        branchKeyStoreArn := "HierarchicalKeyringTestTable",
+        ttlSeconds := ttl,
+        maxCacheSize := Option.Some(10),
+        grantTokens := Option.None
+      )
+    );
+    
+    expect hierarchyKeyringResult.Success?;
+    var hierarchyKeyring := hierarchyKeyringResult.value;
+    
+    var encryptionContext := TestUtils.SmallEncryptionContext(TestUtils.SmallEncryptionContextVariation.A);
+    
+    var algorithmSuiteId := Types.AlgorithmSuiteId.ESDK(Types.ALG_AES_256_GCM_IV12_TAG16_NO_KDF);
+    var encryptionMaterialsIn :- expect mpl.InitializeEncryptionMaterials(
+      Types.InitializeEncryptionMaterialsInput(
+        algorithmSuiteId := algorithmSuiteId,
+        encryptionContext := encryptionContext,
+        signingKey := None,
+        verificationKey := None
+      )
+    );
+
+    var encryptionMaterialsOut :- expect hierarchyKeyring.OnEncrypt(
+      Types.OnEncryptInput(materials:=encryptionMaterialsIn)
+    );
+    
+    var _ :- expect mpl.EncryptionMaterialsHasPlaintextDataKey(encryptionMaterialsOut.materials);
+
+    expect |encryptionMaterialsOut.materials.encryptedDataKeys| == 1;
+
+    var edk := encryptionMaterialsOut.materials.encryptedDataKeys[0];
+
+    var decryptionMaterialsIn :- expect mpl.InitializeDecryptionMaterials(
+      Types.InitializeDecryptionMaterialsInput(
+        algorithmSuiteId := algorithmSuiteId,
+        encryptionContext := encryptionContext
+      )
+    );
+    var decryptionMaterialsOut :- expect hierarchyKeyring.OnDecrypt(
+      Types.OnDecryptInput(
+        materials:=decryptionMaterialsIn,
+        encryptedDataKeys:=[edk]
+      )
+    );
+
+    //= compliance/framework/raw-aes-keyring.txt#2.7.2
+    //= type=test
+    //# If a decryption succeeds, this keyring MUST add the resulting
+    //# plaintext data key to the decryption materials and return the
+    //# modified materials.
+    expect encryptionMaterialsOut.materials.plaintextDataKey
+    == decryptionMaterialsOut.materials.plaintextDataKey;
+  }
+}
