AwsCryptographicMaterialProviders/Model/ddb.smithy
@@ -4,6 +4,11 @@ use aws.polymorph#reference
 
 use com.amazonaws.dynamodb#DynamoDB_20120810
 
+///////////////////
+// Basic structures
+
+string DdbTableArn
+
 ///////////
 // Clients
 
