model/traits.smithy
@@ -57,21 +57,6 @@ structure dafnyUtf8Bytes {}
 @trait(selector: "resource")
 structure extendable {}
 
-// A trait indicating that a structure is a members of a union
-// and MUST NOT be used independently of the union.
-// This is syntactic sugar for
-//  union Foo {
-//    Bar: structure Bar { baz: String }
-//  }
-//
-// It is used like this
-//  union Foo {
-//    Bar: Bar
-//  }
-//  structure Bar { baz: String }
-// This is especilay useful in Dafny.
-// Because it results in a single datatype
-// whos constructors are the member structures.
-// datatypes Foo = Bar( baz: String )
-@trait(selector: "structure")
-structure datatypeUnion {}
+// A trait to indicate that a resource stores local state
+@trait(selector: "resource")
+structure mutableLocalState {}
